<?xml version="1.0"?>
<rdf:RDF xmlns="http://purl.obolibrary.org/obo/foodon/imports/wine_pasta.owl#"
     xml:base="http://purl.obolibrary.org/obo/foodon/imports/wine_pasta.owl"
     xmlns:obo="http://purl.obolibrary.org/obo/"
     xmlns:owl="http://www.w3.org/2002/07/owl#"
     xmlns:rdf="http://www.w3.org/1999/02/22-rdf-syntax-ns#"
     xmlns:xml="http://www.w3.org/XML/1998/namespace"
     xmlns:xsd="http://www.w3.org/2001/XMLSchema#"
     xmlns:rdfs="http://www.w3.org/2000/01/rdf-schema#"
     xmlns:schema="http://schema.org/"
     xmlns:oboInOwl="http://www.geneontology.org/formats/oboInOwl#">
    <owl:Ontology rdf:about="http://purl.obolibrary.org/obo/foodon/imports/wine_pasta.owl"/>
    


    <!-- 
    ///////////////////////////////////////////////////////////////////////////////////////
    //
    // Annotation properties
    //
    ///////////////////////////////////////////////////////////////////////////////////////
     -->

    


    <!-- http://purl.obolibrary.org/obo/IAO_0000114 -->

    <owl:AnnotationProperty rdf:about="http://purl.obolibrary.org/obo/IAO_0000114"/>
    


    <!-- http://purl.obolibrary.org/obo/IAO_0000115 -->

    <owl:AnnotationProperty rdf:about="http://purl.obolibrary.org/obo/IAO_0000115"/>
    


    <!-- http://purl.obolibrary.org/obo/IAO_0000117 -->

    <owl:AnnotationProperty rdf:about="http://purl.obolibrary.org/obo/IAO_0000117"/>
    


    <!-- http://purl.obolibrary.org/obo/IAO_0000119 -->

    <owl:AnnotationProperty rdf:about="http://purl.obolibrary.org/obo/IAO_0000119"/>
    


    <!-- http://schema.org/image -->

    <owl:AnnotationProperty rdf:about="http://schema.org/image"/>
    


    <!-- http://www.geneontology.org/formats/oboInOwl#hasExactSynonym -->

    <owl:AnnotationProperty rdf:about="http://www.geneontology.org/formats/oboInOwl#hasExactSynonym"/>
    


    <!-- 
    ///////////////////////////////////////////////////////////////////////////////////////
    //
    // Object Properties
    //
    ///////////////////////////////////////////////////////////////////////////////////////
     -->

    


    <!-- http://purl.obolibrary.org/obo/RO_0001000 -->

    <owl:ObjectProperty rdf:about="http://purl.obolibrary.org/obo/RO_0001000"/>
    


    <!-- 
    ///////////////////////////////////////////////////////////////////////////////////////
    //
    // Classes
    //
    ///////////////////////////////////////////////////////////////////////////////////////
     -->

    


    <!-- http://purl.obolibrary.org/obo/FOODON_00001211 -->

    <owl:Class rdf:about="http://purl.obolibrary.org/obo/FOODON_00001211"/>
    


    <!-- http://purl.obolibrary.org/obo/FOODON_00002577 -->

    <owl:Class rdf:about="http://purl.obolibrary.org/obo/FOODON_00002577"/>
    


    <!-- http://purl.obolibrary.org/obo/FOODON_00002583 -->

    <owl:Class rdf:about="http://purl.obolibrary.org/obo/FOODON_00002583">
        <rdfs:subClassOf rdf:resource="http://purl.obolibrary.org/obo/FOODON_03412121"/>
        <obo:IAO_0000115 xml:lang="en">The Chardonnay grape plant is the result of a cross between the Pinot noir and Gouais blanc (Heunisch) grape varieties. It produces a green-skinned grape variety used in the production of white wine.</obo:IAO_0000115>
        <obo:IAO_0000119 rdf:datatype="http://www.w3.org/2001/XMLSchema#string">https://en.wikipedia.org/wiki/Chardonnay</obo:IAO_0000119>
        <rdfs:label xml:lang="en">Chardonnay grape plant</rdfs:label>
    </owl:Class>
    


    <!-- http://purl.obolibrary.org/obo/FOODON_00002584 -->

    <owl:Class rdf:about="http://purl.obolibrary.org/obo/FOODON_00002584">
        <rdfs:subClassOf rdf:resource="http://purl.obolibrary.org/obo/FOODON_03310273"/>
        <rdfs:subClassOf>
            <owl:Class>
                <owl:intersectionOf rdf:parseType="Collection">
                    <owl:Restriction>
                        <owl:onProperty rdf:resource="http://purl.obolibrary.org/obo/RO_0001000"/>
                        <owl:someValuesFrom rdf:resource="http://purl.obolibrary.org/obo/FOODON_00002583"/>
                    </owl:Restriction>
                    <owl:Restriction>
                        <owl:onProperty rdf:resource="http://purl.obolibrary.org/obo/RO_0001000"/>
                        <owl:allValuesFrom rdf:resource="http://purl.obolibrary.org/obo/FOODON_00002583"/>
                    </owl:Restriction>
                </owl:intersectionOf>
            </owl:Class>
        </rdfs:subClassOf>
        <obo:IAO_0000114 rdf:resource="http://purl.obolibrary.org/obo/IAO_0000122"/>
        <obo:IAO_0000115 xml:lang="en">Chardonnay wine is wine produced using only Chardonnay grapes.</obo:IAO_0000115>
        <obo:IAO_0000117 rdf:datatype="http://www.w3.org/2001/XMLSchema#string">Emma Griffiths</obo:IAO_0000117>
        <obo:IAO_0000119 rdf:datatype="http://www.w3.org/2001/XMLSchema#string">https://en.wikipedia.org/wiki/Chardonnay</obo:IAO_0000119>
        <rdfs:label xml:lang="en">Chardonnay wine</rdfs:label>
    </owl:Class>
    


    <!-- http://purl.obolibrary.org/obo/FOODON_00002585 -->

    <owl:Class rdf:about="http://purl.obolibrary.org/obo/FOODON_00002585">
        <rdfs:subClassOf rdf:resource="http://purl.obolibrary.org/obo/FOODON_03310272"/>
        <rdfs:subClassOf>
            <owl:Class>
                <owl:intersectionOf rdf:parseType="Collection">
                    <owl:Restriction>
                        <owl:onProperty rdf:resource="http://purl.obolibrary.org/obo/RO_0001000"/>
                        <owl:someValuesFrom rdf:resource="http://purl.obolibrary.org/obo/FOODON_00002640"/>
                    </owl:Restriction>
                    <owl:Restriction>
                        <owl:onProperty rdf:resource="http://purl.obolibrary.org/obo/RO_0001000"/>
                        <owl:allValuesFrom rdf:resource="http://purl.obolibrary.org/obo/FOODON_00002640"/>
                    </owl:Restriction>
                </owl:intersectionOf>
            </owl:Class>
        </rdfs:subClassOf>
        <obo:IAO_0000114 rdf:resource="http://purl.obolibrary.org/obo/IAO_0000122"/>
        <obo:IAO_0000115 xml:lang="en">A Cabernet Sauvignon wine is any wine produced using only Cabernet Sauvignon grapes. It often appears with Merlot and Cabernet Franc in blended Bordeaux wines.</obo:IAO_0000115>
        <obo:IAO_0000117 rdf:datatype="http://www.w3.org/2001/XMLSchema#string">Damion Dooley</obo:IAO_0000117>
        <obo:IAO_0000119 rdf:datatype="http://www.w3.org/2001/XMLSchema#string">https://en.wikipedia.org/wiki/Cabernet_Sauvignon</obo:IAO_0000119>
        <rdfs:label xml:lang="en">Cabernet Sauvignon wine</rdfs:label>
    </owl:Class>
    


    <!-- http://purl.obolibrary.org/obo/FOODON_00002586 -->

    <owl:Class rdf:about="http://purl.obolibrary.org/obo/FOODON_00002586">
        <rdfs:subClassOf rdf:resource="http://purl.obolibrary.org/obo/FOODON_03310273"/>
        <rdfs:subClassOf>
            <owl:Class>
                <owl:intersectionOf rdf:parseType="Collection">
                    <owl:Restriction>
                        <owl:onProperty rdf:resource="http://purl.obolibrary.org/obo/RO_0001000"/>
                        <owl:someValuesFrom rdf:resource="http://purl.obolibrary.org/obo/FOODON_00002587"/>
                    </owl:Restriction>
                    <owl:Restriction>
                        <owl:onProperty rdf:resource="http://purl.obolibrary.org/obo/RO_0001000"/>
                        <owl:allValuesFrom rdf:resource="http://purl.obolibrary.org/obo/FOODON_00002587"/>
                    </owl:Restriction>
                </owl:intersectionOf>
            </owl:Class>
        </rdfs:subClassOf>
        <obo:IAO_0000114 rdf:resource="http://purl.obolibrary.org/obo/IAO_0000122"/>
        <obo:IAO_0000115 xml:lang="en">A Chenin blanc wine is any wine produced using only Chenin blanc grapes.</obo:IAO_0000115>
        <obo:IAO_0000117 rdf:datatype="http://www.w3.org/2001/XMLSchema#string">Lauren Tindale</obo:IAO_0000117>
        <rdfs:label xml:lang="en">Chenin blanc wine</rdfs:label>
    </owl:Class>
    


    <!-- http://purl.obolibrary.org/obo/FOODON_00002587 -->

    <owl:Class rdf:about="http://purl.obolibrary.org/obo/FOODON_00002587">
        <rdfs:subClassOf rdf:resource="http://purl.obolibrary.org/obo/FOODON_03412121"/>
        <obo:IAO_0000114 rdf:resource="http://purl.obolibrary.org/obo/IAO_0000122"/>
        <obo:IAO_0000115 xml:lang="en">Chenin blanc grapes are a White wine grape variety from the Loire Valley of France. Its high acidity means it can be used to make everything from sparkling wines to well-balanced dessert wines, although it can produce very bland, neutral wines if the vine&apos;s natural vigor is not controlled.</obo:IAO_0000115>
        <obo:IAO_0000117 rdf:datatype="http://www.w3.org/2001/XMLSchema#string">Lauren Tindale</obo:IAO_0000117>
        <obo:IAO_0000119 rdf:datatype="http://www.w3.org/2001/XMLSchema#string">https://en.wikipedia.org/wiki/Chenin_blanc</obo:IAO_0000119>
        <oboInOwl:hasExactSynonym xml:lang="fr">Pineau de la Loire</oboInOwl:hasExactSynonym>
        <rdfs:label xml:lang="en">Chenin blanc grape plant</rdfs:label>
    </owl:Class>
    


    <!-- http://purl.obolibrary.org/obo/FOODON_00002588 -->

    <owl:Class rdf:about="http://purl.obolibrary.org/obo/FOODON_00002588">
        <rdfs:subClassOf rdf:resource="http://purl.obolibrary.org/obo/FOODON_03310272"/>
        <rdfs:subClassOf>
            <owl:Class>
                <owl:intersectionOf rdf:parseType="Collection">
                    <owl:Restriction>
                        <owl:onProperty rdf:resource="http://purl.obolibrary.org/obo/RO_0001000"/>
                        <owl:someValuesFrom rdf:resource="http://purl.obolibrary.org/obo/FOODON_00002589"/>
                    </owl:Restriction>
                    <owl:Restriction>
                        <owl:onProperty rdf:resource="http://purl.obolibrary.org/obo/RO_0001000"/>
                        <owl:allValuesFrom rdf:resource="http://purl.obolibrary.org/obo/FOODON_00002589"/>
                    </owl:Restriction>
                </owl:intersectionOf>
            </owl:Class>
        </rdfs:subClassOf>
        <obo:IAO_0000114 rdf:resource="http://purl.obolibrary.org/obo/IAO_0000122"/>
        <obo:IAO_0000115 xml:lang="en">A Malbec wine is any wine produced using only Malbec grapes.</obo:IAO_0000115>
        <obo:IAO_0000117 rdf:datatype="http://www.w3.org/2001/XMLSchema#string">Lauren Tindale</obo:IAO_0000117>
        <rdfs:label xml:lang="en">Malbec wine</rdfs:label>
    </owl:Class>
    


    <!-- http://purl.obolibrary.org/obo/FOODON_00002589 -->

    <owl:Class rdf:about="http://purl.obolibrary.org/obo/FOODON_00002589">
        <rdfs:subClassOf rdf:resource="http://purl.obolibrary.org/obo/FOODON_03412121"/>
        <obo:IAO_0000114 rdf:resource="http://purl.obolibrary.org/obo/IAO_0000122"/>
        <obo:IAO_0000115 xml:lang="en">Malbec grapes are a purple grape variety used in making red wine. The grapes tend to have an inky dark color and robust tannins, and are known as one of the six grapes allowed in the blend of red Bordeaux wine. The French plantations of Malbec are now found primarily in Cahors in South West France. It is increasingly celebrated as an Argentine varietal wine and is being grown around the world.</obo:IAO_0000115>
        <obo:IAO_0000117 rdf:datatype="http://www.w3.org/2001/XMLSchema#string">Lauren Tindale</obo:IAO_0000117>
        <obo:IAO_0000119 rdf:datatype="http://www.w3.org/2001/XMLSchema#string">https://en.wikipedia.org/wiki/Malbec</obo:IAO_0000119>
        <rdfs:label xml:lang="en">Malbec grape plant</rdfs:label>
    </owl:Class>
    


    <!-- http://purl.obolibrary.org/obo/FOODON_00002590 -->

    <owl:Class rdf:about="http://purl.obolibrary.org/obo/FOODON_00002590">
        <rdfs:subClassOf rdf:resource="http://purl.obolibrary.org/obo/FOODON_03310272"/>
        <rdfs:subClassOf>
            <owl:Class>
                <owl:intersectionOf rdf:parseType="Collection">
                    <owl:Restriction>
                        <owl:onProperty rdf:resource="http://purl.obolibrary.org/obo/RO_0001000"/>
                        <owl:someValuesFrom rdf:resource="http://purl.obolibrary.org/obo/FOODON_00002591"/>
                    </owl:Restriction>
                    <owl:Restriction>
                        <owl:onProperty rdf:resource="http://purl.obolibrary.org/obo/RO_0001000"/>
                        <owl:allValuesFrom rdf:resource="http://purl.obolibrary.org/obo/FOODON_00002591"/>
                    </owl:Restriction>
                </owl:intersectionOf>
            </owl:Class>
        </rdfs:subClassOf>
        <obo:IAO_0000114 rdf:resource="http://purl.obolibrary.org/obo/IAO_0000122"/>
        <obo:IAO_0000115 xml:lang="en">A Merlot wine is any wine produced using only Merlot grapes.</obo:IAO_0000115>
        <obo:IAO_0000117 rdf:datatype="http://www.w3.org/2001/XMLSchema#string">Lauren Tindale</obo:IAO_0000117>
        <rdfs:label xml:lang="en">Merlot wine</rdfs:label>
    </owl:Class>
    


    <!-- http://purl.obolibrary.org/obo/FOODON_00002591 -->

    <owl:Class rdf:about="http://purl.obolibrary.org/obo/FOODON_00002591">
        <rdfs:subClassOf rdf:resource="http://purl.obolibrary.org/obo/FOODON_03412121"/>
        <obo:IAO_0000114 rdf:resource="http://purl.obolibrary.org/obo/IAO_0000122"/>
        <obo:IAO_0000115 xml:lang="en">Merlot is a dark blue-colored wine grape variety, that is used as both a blending grape and for varietal wines.</obo:IAO_0000115>
        <obo:IAO_0000117 rdf:datatype="http://www.w3.org/2001/XMLSchema#string">Lauren Tindale</obo:IAO_0000117>
        <obo:IAO_0000119 rdf:datatype="http://www.w3.org/2001/XMLSchema#string">https://en.wikipedia.org/wiki/Merlot</obo:IAO_0000119>
        <schema:image rdf:resource="https://upload.wikimedia.org/wikipedia/commons/thumb/e/ee/Merlot_Grape.jpg/320px-Merlot_Grape.jpg"/>
        <rdfs:label xml:lang="en">Merlot grape plant</rdfs:label>
    </owl:Class>
    


    <!-- http://purl.obolibrary.org/obo/FOODON_00002592 -->

    <owl:Class rdf:about="http://purl.obolibrary.org/obo/FOODON_00002592">
        <rdfs:subClassOf rdf:resource="http://purl.obolibrary.org/obo/FOODON_03310273"/>
        <rdfs:subClassOf>
            <owl:Class>
                <owl:intersectionOf rdf:parseType="Collection">
                    <owl:Restriction>
                        <owl:onProperty rdf:resource="http://purl.obolibrary.org/obo/RO_0001000"/>
                        <owl:someValuesFrom rdf:resource="http://purl.obolibrary.org/obo/FOODON_00002593"/>
                    </owl:Restriction>
                    <owl:Restriction>
                        <owl:onProperty rdf:resource="http://purl.obolibrary.org/obo/RO_0001000"/>
                        <owl:allValuesFrom rdf:resource="http://purl.obolibrary.org/obo/FOODON_00002593"/>
                    </owl:Restriction>
                </owl:intersectionOf>
            </owl:Class>
        </rdfs:subClassOf>
        <obo:IAO_0000114 rdf:resource="http://purl.obolibrary.org/obo/IAO_0000122"/>
        <obo:IAO_0000115 xml:lang="en">A pinot blanc wine is any wine produced using only Pinco blanc grapes.</obo:IAO_0000115>
        <obo:IAO_0000117 rdf:datatype="http://www.w3.org/2001/XMLSchema#string">Lauren Tindale</obo:IAO_0000117>
        <rdfs:label xml:lang="en">Pinot blanc wine</rdfs:label>
    </owl:Class>
    


    <!-- http://purl.obolibrary.org/obo/FOODON_00002593 -->

    <owl:Class rdf:about="http://purl.obolibrary.org/obo/FOODON_00002593">
        <rdfs:subClassOf rdf:resource="http://purl.obolibrary.org/obo/FOODON_03412121"/>
        <obo:IAO_0000114 rdf:resource="http://purl.obolibrary.org/obo/IAO_0000122"/>
        <obo:IAO_0000115 xml:lang="en">Pinot blanc is a white wine grape. It is a point genetic mutation of Pinot noir.</obo:IAO_0000115>
        <obo:IAO_0000117 rdf:datatype="http://www.w3.org/2001/XMLSchema#string">Lauren Tindale</obo:IAO_0000117>
        <obo:IAO_0000119 rdf:datatype="http://www.w3.org/2001/XMLSchema#string">https://en.wikipedia.org/wiki/Pinot_blanc</obo:IAO_0000119>
        <schema:image rdf:resource="https://upload.wikimedia.org/wikipedia/commons/thumb/b/b3/Pinot-blanc.jpg/440px-Pinot-blanc.jpg"/>
        <rdfs:label xml:lang="en">Pinot blanc grape plant</rdfs:label>
    </owl:Class>
    


    <!-- http://purl.obolibrary.org/obo/FOODON_00002594 -->

    <owl:Class rdf:about="http://purl.obolibrary.org/obo/FOODON_00002594">
        <rdfs:subClassOf rdf:resource="http://purl.obolibrary.org/obo/FOODON_03310273"/>
        <rdfs:subClassOf>
            <owl:Class>
                <owl:intersectionOf rdf:parseType="Collection">
                    <owl:Restriction>
                        <owl:onProperty rdf:resource="http://purl.obolibrary.org/obo/RO_0001000"/>
                        <owl:someValuesFrom rdf:resource="http://purl.obolibrary.org/obo/FOODON_00002595"/>
                    </owl:Restriction>
                    <owl:Restriction>
                        <owl:onProperty rdf:resource="http://purl.obolibrary.org/obo/RO_0001000"/>
                        <owl:allValuesFrom rdf:resource="http://purl.obolibrary.org/obo/FOODON_00002595"/>
                    </owl:Restriction>
                </owl:intersectionOf>
            </owl:Class>
        </rdfs:subClassOf>
        <obo:IAO_0000114 rdf:resource="http://purl.obolibrary.org/obo/IAO_0000122"/>
        <obo:IAO_0000115 xml:lang="en">Pinot gris is a white wine varietal produced only from Pinot gris grapes.  The Italian synonym, Pinot Grigio, has become strongly associated with lighter wines produced in great quantities, particularly in northern Italy.</obo:IAO_0000115>
        <obo:IAO_0000117 rdf:datatype="http://www.w3.org/2001/XMLSchema#string">Ginny Pichler</obo:IAO_0000117>
        <obo:IAO_0000119 rdf:datatype="http://www.w3.org/2001/XMLSchema#string">https://www.wine-searcher.com/grape-381-pinot-grigio</obo:IAO_0000119>
        <schema:image rdf:resource="https://upload.wikimedia.org/wikipedia/commons/thumb/5/59/Alto_adige_Pinot_grigio.jpg/179px-Alto_adige_Pinot_grigio.jpg"/>
        <oboInOwl:hasExactSynonym xml:lang="ge">Grauburgunder</oboInOwl:hasExactSynonym>
        <oboInOwl:hasExactSynonym xml:lang="it">Pinot Grigio</oboInOwl:hasExactSynonym>
        <rdfs:label xml:lang="en">Pinot gris wine</rdfs:label>
    </owl:Class>
    


    <!-- http://purl.obolibrary.org/obo/FOODON_00002595 -->

    <owl:Class rdf:about="http://purl.obolibrary.org/obo/FOODON_00002595">
        <rdfs:subClassOf rdf:resource="http://purl.obolibrary.org/obo/FOODON_03412121"/>
        <obo:IAO_0000114 rdf:resource="http://purl.obolibrary.org/obo/IAO_0000122"/>
        <obo:IAO_0000115 xml:lang="en">Pinot gris is a white wine grape variety (mutation) of the Pinot family which shares its genetic fingerprint with Pinot Noir, Pinot Blanc et al. . Pinot gris is grown around the globe with the &quot;spicy&quot; full-bodied Alsatian and lighter-bodied, more acidic Italian styles being most widely recognized.</obo:IAO_0000115>
        <obo:IAO_0000117 rdf:datatype="http://www.w3.org/2001/XMLSchema#string">Ginny Pichler</obo:IAO_0000117>
        <obo:IAO_0000119 rdf:datatype="http://www.w3.org/2001/XMLSchema#string">https://en.wikipedia.org/wiki/Pinot_gris</obo:IAO_0000119>
        <schema:image rdf:resource="https://commons.wikimedia.org/wiki/File:Pinot_Gris_close.JPG"/>
        <oboInOwl:hasExactSynonym xml:lang="ge">Grauburgunder</oboInOwl:hasExactSynonym>
        <oboInOwl:hasExactSynonym xml:lang="it">Pinot Grigio grape</oboInOwl:hasExactSynonym>
        <rdfs:label xml:lang="en">Pinot gris grape plant</rdfs:label>
    </owl:Class>
    


    <!-- http://purl.obolibrary.org/obo/FOODON_00002596 -->

    <owl:Class rdf:about="http://purl.obolibrary.org/obo/FOODON_00002596">
        <rdfs:subClassOf rdf:resource="http://purl.obolibrary.org/obo/FOODON_03310272"/>
        <rdfs:subClassOf>
            <owl:Class>
                <owl:intersectionOf rdf:parseType="Collection">
                    <owl:Restriction>
                        <owl:onProperty rdf:resource="http://purl.obolibrary.org/obo/RO_0001000"/>
                        <owl:someValuesFrom rdf:resource="http://purl.obolibrary.org/obo/FOODON_00002597"/>
                    </owl:Restriction>
                    <owl:Restriction>
                        <owl:onProperty rdf:resource="http://purl.obolibrary.org/obo/RO_0001000"/>
                        <owl:allValuesFrom rdf:resource="http://purl.obolibrary.org/obo/FOODON_00002597"/>
                    </owl:Restriction>
                </owl:intersectionOf>
            </owl:Class>
        </rdfs:subClassOf>
        <obo:IAO_0000114 rdf:resource="http://purl.obolibrary.org/obo/IAO_0000122"/>
        <obo:IAO_0000115 xml:lang="en">Pinot noir wine is a red wine varietal made only from Pinot noir grapes.  The thin skins and low levels of phenolic compounds lends pinot to producing mostly lightly colored, medium-bodied and low-tannin wines that can often go through phases of uneven and unpredictable aging.</obo:IAO_0000115>
        <obo:IAO_0000117 rdf:datatype="http://www.w3.org/2001/XMLSchema#string">Shannon Russell</obo:IAO_0000117>
        <obo:IAO_0000119 rdf:datatype="http://www.w3.org/2001/XMLSchema#string">https://en.wikipedia.org/wiki/Pinot_noir</obo:IAO_0000119>
        <oboInOwl:hasExactSynonym xml:lang="fr"> Pinot Nero</oboInOwl:hasExactSynonym>
        <oboInOwl:hasExactSynonym xml:lang="ge"> Spätburgunder</oboInOwl:hasExactSynonym>
        <oboInOwl:hasExactSynonym xml:lang="ge">Blauburgunder </oboInOwl:hasExactSynonym>
        <oboInOwl:hasExactSynonym xml:lang="fr">Rulandské modré </oboInOwl:hasExactSynonym>
        <rdfs:label xml:lang="en">Pinot noir wine</rdfs:label>
    </owl:Class>
    


    <!-- http://purl.obolibrary.org/obo/FOODON_00002597 -->

    <owl:Class rdf:about="http://purl.obolibrary.org/obo/FOODON_00002597">
        <rdfs:subClassOf rdf:resource="http://purl.obolibrary.org/obo/FOODON_03412121"/>
        <obo:IAO_0000114 rdf:resource="http://purl.obolibrary.org/obo/IAO_0000122"/>
        <obo:IAO_0000115 xml:lang="en">Pinot noir grape is a red wine grape variety. The name is derived from the French words for pine and black. The word pine alludes to the grape variety having tightly clustered, pine cone-shaped bunches of fruit. Pinot noir grapes are grown around the world, mostly in the cooler climates, and the grape is chiefly associated with the Burgundy region of France.</obo:IAO_0000115>
        <obo:IAO_0000117 rdf:datatype="http://www.w3.org/2001/XMLSchema#string">Shannon Russell</obo:IAO_0000117>
        <obo:IAO_0000119 rdf:datatype="http://www.w3.org/2001/XMLSchema#string">https://en.wikipedia.org/wiki/Pinot_noir</obo:IAO_0000119>
        <schema:image rdf:resource="https://en.wikipedia.org/wiki/Pinot_noir#/media/File:Grape_near_Sancerre.jpg"/>
        <rdfs:label xml:lang="en">Pinot noir grape plant</rdfs:label>
    </owl:Class>
    


    <!-- http://purl.obolibrary.org/obo/FOODON_00002598 -->

    <owl:Class rdf:about="http://purl.obolibrary.org/obo/FOODON_00002598">
        <rdfs:subClassOf rdf:resource="http://purl.obolibrary.org/obo/FOODON_03310272"/>
        <rdfs:subClassOf>
            <owl:Class>
                <owl:intersectionOf rdf:parseType="Collection">
                    <owl:Restriction>
                        <owl:onProperty rdf:resource="http://purl.obolibrary.org/obo/RO_0001000"/>
                        <owl:someValuesFrom rdf:resource="http://purl.obolibrary.org/obo/FOODON_00002599"/>
                    </owl:Restriction>
                    <owl:Restriction>
                        <owl:onProperty rdf:resource="http://purl.obolibrary.org/obo/RO_0001000"/>
                        <owl:allValuesFrom rdf:resource="http://purl.obolibrary.org/obo/FOODON_00002599"/>
                    </owl:Restriction>
                </owl:intersectionOf>
            </owl:Class>
        </rdfs:subClassOf>
        <obo:IAO_0000114 rdf:resource="http://purl.obolibrary.org/obo/IAO_0000122"/>
        <obo:IAO_0000115 xml:lang="en">Pinotage wine is a red wine varietal produced only from Pinotage grapes. This type of wine can range from a fairly cheap, light-bodied red wine with some funky aromas (including extremes such as acetone, paint, rubber, and at times banana) all the way to full-bodied red wines with balance, elegance, fully developed black fruit flavors, and an enduring, sweet, smokey finish.</obo:IAO_0000115>
        <obo:IAO_0000117 rdf:datatype="http://www.w3.org/2001/XMLSchema#string">Ginny Pichler</obo:IAO_0000117>
        <obo:IAO_0000119 rdf:datatype="http://www.w3.org/2001/XMLSchema#string">https://www.thespruceeats.com/what-is-pinotage-wine-3511226</obo:IAO_0000119>
        <schema:image rdf:resource="https://upload.wikimedia.org/wikipedia/commons/thumb/e/e4/Stellenbosch_Pinotage.jpg/179px-Stellenbosch_Pinotage.jpg"/>
        <rdfs:label xml:lang="en">Pinotage wine</rdfs:label>
    </owl:Class>
    


    <!-- http://purl.obolibrary.org/obo/FOODON_00002599 -->

    <owl:Class rdf:about="http://purl.obolibrary.org/obo/FOODON_00002599">
        <rdfs:subClassOf rdf:resource="http://purl.obolibrary.org/obo/FOODON_03412121"/>
        <obo:IAO_0000114 rdf:resource="http://purl.obolibrary.org/obo/IAO_0000122"/>
        <obo:IAO_0000115 xml:lang="en">Pinotage is a red wine grape that is South Africa&apos;s signature variety. It was bred there in 1925 as a crossbetween Pinot noir and Cinsaut. The grape is a viticultural intraspecific cross of two varieties of Vitis vinifera, not an interspecific hybrid.</obo:IAO_0000115>
        <obo:IAO_0000117 rdf:datatype="http://www.w3.org/2001/XMLSchema#string">Ginny Pichler</obo:IAO_0000117>
        <obo:IAO_0000119 rdf:datatype="http://www.w3.org/2001/XMLSchema#string">https://en.wikipedia.org/wiki/Pinotage</obo:IAO_0000119>
        <schema:image rdf:resource="https://i2.wp.com/www.winetwofive.com/wp-content/uploads/2018/06/CEP-TIBOUREN.jpg?resize=128%2C128"/>
        <rdfs:label xml:lang="en">Pinotage grape plant</rdfs:label>
    </owl:Class>
    


    <!-- http://purl.obolibrary.org/obo/FOODON_00002600 -->

    <owl:Class rdf:about="http://purl.obolibrary.org/obo/FOODON_00002600">
        <rdfs:subClassOf rdf:resource="http://purl.obolibrary.org/obo/FOODON_03301014"/>
        <obo:IAO_0000114 rdf:resource="http://purl.obolibrary.org/obo/IAO_0000122"/>
        <obo:IAO_0000115 xml:lang="en">Reserve wine is wine of a higher quality than usual, or a wine that has been aged before being sold, or both. Traditionally, winemakers would reserve some of their best wine rather than sell it immediately, coining the term.</obo:IAO_0000115>
        <obo:IAO_0000117 rdf:datatype="http://www.w3.org/2001/XMLSchema#string">Damion Dooley</obo:IAO_0000117>
        <obo:IAO_0000119 rdf:datatype="http://www.w3.org/2001/XMLSchema#string">https://en.wikipedia.org/wiki/Reserve_wine</obo:IAO_0000119>
        <rdfs:label xml:lang="en">Reserve wine</rdfs:label>
    </owl:Class>
    


    <!-- http://purl.obolibrary.org/obo/FOODON_00002601 -->

    <owl:Class rdf:about="http://purl.obolibrary.org/obo/FOODON_00002601">
        <rdfs:subClassOf rdf:resource="http://purl.obolibrary.org/obo/FOODON_03310273"/>
        <rdfs:subClassOf>
            <owl:Class>
                <owl:intersectionOf rdf:parseType="Collection">
                    <owl:Restriction>
                        <owl:onProperty rdf:resource="http://purl.obolibrary.org/obo/RO_0001000"/>
                        <owl:someValuesFrom rdf:resource="http://purl.obolibrary.org/obo/FOODON_00002602"/>
                    </owl:Restriction>
                    <owl:Restriction>
                        <owl:onProperty rdf:resource="http://purl.obolibrary.org/obo/RO_0001000"/>
                        <owl:allValuesFrom rdf:resource="http://purl.obolibrary.org/obo/FOODON_00002602"/>
                    </owl:Restriction>
                </owl:intersectionOf>
            </owl:Class>
        </rdfs:subClassOf>
        <obo:IAO_0000114 rdf:resource="http://purl.obolibrary.org/obo/IAO_0000122"/>
        <obo:IAO_0000115 xml:lang="en">Riesling wine is a white wine varietal produced only from Riesling grapes, and offered as dry, semi-sweet, sweet, and sparkling white wines. Riesling wines are usually varietally pure and are seldom oaked. </obo:IAO_0000115>
        <obo:IAO_0000117 rdf:datatype="http://www.w3.org/2001/XMLSchema#string">Ginny Pichler</obo:IAO_0000117>
        <obo:IAO_0000119 rdf:datatype="http://www.w3.org/2001/XMLSchema#string">https://en.wikipedia.org/wiki/Riesling</obo:IAO_0000119>
        <schema:image rdf:resource="https://upload.wikimedia.org/wikipedia/commons/thumb/9/96/Alsatian_Riesling_.jpg/179px-Alsatian_Riesling_.jpg"/>
        <rdfs:label xml:lang="en">Riesling wine</rdfs:label>
    </owl:Class>
    


    <!-- http://purl.obolibrary.org/obo/FOODON_00002602 -->

    <owl:Class rdf:about="http://purl.obolibrary.org/obo/FOODON_00002602">
        <rdfs:subClassOf rdf:resource="http://purl.obolibrary.org/obo/FOODON_03412121"/>
        <obo:IAO_0000114 rdf:resource="http://purl.obolibrary.org/obo/IAO_0000122"/>
        <obo:IAO_0000115 xml:lang="en">Riesling grape is an aromatic white grape variety displaying flowery, almost perfumed, aromas as well as high acidity.</obo:IAO_0000115>
        <obo:IAO_0000117 rdf:datatype="http://www.w3.org/2001/XMLSchema#string">Ginny Pichler</obo:IAO_0000117>
        <obo:IAO_0000119 rdf:datatype="http://www.w3.org/2001/XMLSchema#string">https://en.wikipedia.org/wiki/Riesling</obo:IAO_0000119>
        <schema:image rdf:resource="https://upload.wikimedia.org/wikipedia/commons/thumb/7/76/Riesling_grapes_leaves.jpg/320px-Riesling_grapes_leaves.jpg"/>
        <rdfs:label xml:lang="en">Riesling grape plant</rdfs:label>
    </owl:Class>
    


    <!-- http://purl.obolibrary.org/obo/FOODON_00002603 -->

    <owl:Class rdf:about="http://purl.obolibrary.org/obo/FOODON_00002603">
        <rdfs:subClassOf rdf:resource="http://purl.obolibrary.org/obo/FOODON_03310272"/>
        <rdfs:subClassOf>
            <owl:Class>
                <owl:intersectionOf rdf:parseType="Collection">
                    <owl:Restriction>
                        <owl:onProperty rdf:resource="http://purl.obolibrary.org/obo/RO_0001000"/>
                        <owl:someValuesFrom rdf:resource="http://purl.obolibrary.org/obo/FOODON_00002604"/>
                    </owl:Restriction>
                    <owl:Restriction>
                        <owl:onProperty rdf:resource="http://purl.obolibrary.org/obo/RO_0001000"/>
                        <owl:allValuesFrom rdf:resource="http://purl.obolibrary.org/obo/FOODON_00002604"/>
                    </owl:Restriction>
                </owl:intersectionOf>
            </owl:Class>
        </rdfs:subClassOf>
        <obo:IAO_0000114 rdf:resource="http://purl.obolibrary.org/obo/IAO_0000122"/>
        <obo:IAO_0000115 xml:lang="en">Sangiovese wine is a red wine varietal produced only from Sangiovese grapes. It is prized for its high acid, firm tannins and balanced nature. Savory flavors of dark cherries and black stonefruit are characteristic, and may be backed by secondary notes of tomato leaf and dried herbs.</obo:IAO_0000115>
        <obo:IAO_0000117 rdf:datatype="http://www.w3.org/2001/XMLSchema#string">Ginny Pichler</obo:IAO_0000117>
        <obo:IAO_0000119 rdf:datatype="http://www.w3.org/2001/XMLSchema#string">https://www.wine-searcher.com/grape-432-sangiovese</obo:IAO_0000119>
        <schema:image rdf:resource="https://upload.wikimedia.org/wikipedia/commons/thumb/2/2e/Sangiovese_wine.jpg/180px-Sangiovese_wine.jpg"/>
        <rdfs:label xml:lang="en">Sangiovese wine</rdfs:label>
    </owl:Class>
    


    <!-- http://purl.obolibrary.org/obo/FOODON_00002604 -->

    <owl:Class rdf:about="http://purl.obolibrary.org/obo/FOODON_00002604">
        <rdfs:subClassOf rdf:resource="http://purl.obolibrary.org/obo/FOODON_03412121"/>
        <obo:IAO_0000114 rdf:resource="http://purl.obolibrary.org/obo/IAO_0000122"/>
        <obo:IAO_0000115 xml:lang="en">Sangiovese is a red Italian wine grape variety that derives its name from the Latin sanguis Jovis, &quot;the blood of Jupiter&quot;.</obo:IAO_0000115>
        <obo:IAO_0000117 rdf:datatype="http://www.w3.org/2001/XMLSchema#string">Ginny Pichler</obo:IAO_0000117>
        <obo:IAO_0000119 rdf:datatype="http://www.w3.org/2001/XMLSchema#string">https://en.wikipedia.org/wiki/Sangiovese</obo:IAO_0000119>
        <schema:image rdf:resource="https://upload.wikimedia.org/wikipedia/commons/thumb/3/37/Sangiovese_close_up_crop.jpg/277px-Sangiovese_close_up_crop.jpg"/>
        <rdfs:label xml:lang="en">Sangiovese grape plant</rdfs:label>
    </owl:Class>
    


    <!-- http://purl.obolibrary.org/obo/FOODON_00002605 -->

    <owl:Class rdf:about="http://purl.obolibrary.org/obo/FOODON_00002605">
        <rdfs:subClassOf rdf:resource="http://purl.obolibrary.org/obo/FOODON_03310273"/>
        <rdfs:subClassOf>
            <owl:Class>
                <owl:intersectionOf rdf:parseType="Collection">
                    <owl:Restriction>
                        <owl:onProperty rdf:resource="http://purl.obolibrary.org/obo/RO_0001000"/>
                        <owl:someValuesFrom rdf:resource="http://purl.obolibrary.org/obo/FOODON_00002606"/>
                    </owl:Restriction>
                    <owl:Restriction>
                        <owl:onProperty rdf:resource="http://purl.obolibrary.org/obo/RO_0001000"/>
                        <owl:allValuesFrom rdf:resource="http://purl.obolibrary.org/obo/FOODON_00002606"/>
                    </owl:Restriction>
                </owl:intersectionOf>
            </owl:Class>
        </rdfs:subClassOf>
        <obo:IAO_0000114 rdf:resource="http://purl.obolibrary.org/obo/IAO_0000122"/>
        <obo:IAO_0000115 xml:lang="en">Sauvignon blanc wine is a white wine varietal produced only from Sauvignon blanc grapes.  Its primary fruit flavors are lime, green apple, passion fruit and white peach. Depending on how ripe the grapes are when the wine is made, the flavor will range from zesty lime to flowery peach. </obo:IAO_0000115>
        <obo:IAO_0000117 rdf:datatype="http://www.w3.org/2001/XMLSchema#string">Shannon Russell</obo:IAO_0000117>
        <obo:IAO_0000119 rdf:datatype="http://www.w3.org/2001/XMLSchema#string">https://winefolly.com/review/sauvignon-blanc-wine-taste-food-pairing/</obo:IAO_0000119>
        <oboInOwl:hasExactSynonym xml:lang="fr"> Blanc fume </oboInOwl:hasExactSynonym>
        <oboInOwl:hasExactSynonym xml:lang="fr"> Fume blanc</oboInOwl:hasExactSynonym>
        <oboInOwl:hasExactSynonym xml:lang="en">Muskat-Silvaner</oboInOwl:hasExactSynonym>
        <oboInOwl:hasExactSynonym xml:lang="fr">Sauvignon jaune </oboInOwl:hasExactSynonym>
        <rdfs:label xml:lang="en">Sauvignon blanc wine</rdfs:label>
    </owl:Class>
    


    <!-- http://purl.obolibrary.org/obo/FOODON_00002606 -->

    <owl:Class rdf:about="http://purl.obolibrary.org/obo/FOODON_00002606">
        <rdfs:subClassOf rdf:resource="http://purl.obolibrary.org/obo/FOODON_03412121"/>
        <obo:IAO_0000114 rdf:resource="http://purl.obolibrary.org/obo/IAO_0000122"/>
        <obo:IAO_0000115 xml:lang="en">Sauvignon blanc is a green-skinned grape variety that originates from the Bordeaux region of France. The grape most likely gets its name from the French words sauvage (&quot;wild&quot;) and blanc (&quot;white&quot;) due to its early origins as an indigenous grape in South West France.</obo:IAO_0000115>
        <obo:IAO_0000117 rdf:datatype="http://www.w3.org/2001/XMLSchema#string">Shannon Russell</obo:IAO_0000117>
        <obo:IAO_0000119 rdf:datatype="http://www.w3.org/2001/XMLSchema#string">https://en.wikipedia.org/wiki/Sauvignon_blanc</obo:IAO_0000119>
        <schema:image rdf:resource="https://upload.wikimedia.org/wikipedia/commons/thumb/5/50/Sauvignon_blanc_grapes.jpg/360px-Sauvignon_blanc_grapes.jpg"/>
        <rdfs:label xml:lang="en">Sauvignon blanc grape plant</rdfs:label>
    </owl:Class>
    


    <!-- http://purl.obolibrary.org/obo/FOODON_00002607 -->

    <owl:Class rdf:about="http://purl.obolibrary.org/obo/FOODON_00002607">
        <rdfs:subClassOf rdf:resource="http://purl.obolibrary.org/obo/FOODON_03310273"/>
        <rdfs:subClassOf>
            <owl:Class>
                <owl:intersectionOf rdf:parseType="Collection">
                    <owl:Restriction>
                        <owl:onProperty rdf:resource="http://purl.obolibrary.org/obo/RO_0001000"/>
                        <owl:someValuesFrom rdf:resource="http://purl.obolibrary.org/obo/FOODON_00002608"/>
                    </owl:Restriction>
                    <owl:Restriction>
                        <owl:onProperty rdf:resource="http://purl.obolibrary.org/obo/RO_0001000"/>
                        <owl:allValuesFrom rdf:resource="http://purl.obolibrary.org/obo/FOODON_00002608"/>
                    </owl:Restriction>
                </owl:intersectionOf>
            </owl:Class>
        </rdfs:subClassOf>
        <obo:IAO_0000114 rdf:resource="http://purl.obolibrary.org/obo/IAO_0000122"/>
        <obo:IAO_0000115 xml:lang="en">Semillon wine is a white wine varietal produced only from Semillon grapes.  The primary fruit flavors in Semillon wine are lemon, apple, pear and green papaya. Semillon is France’s 3rd most planted white wine variety behind Sauvignon Blanc and Chardonnay.</obo:IAO_0000115>
        <obo:IAO_0000117 rdf:datatype="http://www.w3.org/2001/XMLSchema#string">Ginny Pichler</obo:IAO_0000117>
        <obo:IAO_0000119 rdf:datatype="http://www.w3.org/2001/XMLSchema#string">https://winefolly.com/review/have-you-heard-of-semillon-the-3rd-most-important-french-white-wine/</obo:IAO_0000119>
        <schema:image rdf:resource="https://upload.wikimedia.org/wikipedia/commons/thumb/1/1d/Late_harvest_Semillon.jpg/179px-Late_harvest_Semillon.jpg"/>
        <oboInOwl:hasExactSynonym xml:lang="fr">Sémillon wine</oboInOwl:hasExactSynonym>
        <rdfs:label xml:lang="en">Semillon wine</rdfs:label>
    </owl:Class>
    


    <!-- http://purl.obolibrary.org/obo/FOODON_00002608 -->

    <owl:Class rdf:about="http://purl.obolibrary.org/obo/FOODON_00002608">
        <rdfs:subClassOf rdf:resource="http://purl.obolibrary.org/obo/FOODON_03412121"/>
        <obo:IAO_0000114 rdf:resource="http://purl.obolibrary.org/obo/IAO_0000122"/>
        <obo:IAO_0000115 xml:lang="en">Semillon is a golden-skinned grape used to make dry and sweet white wines, mostly in France and Australia.</obo:IAO_0000115>
        <obo:IAO_0000117 rdf:datatype="http://www.w3.org/2001/XMLSchema#string">Ginny Pichler</obo:IAO_0000117>
        <obo:IAO_0000119 rdf:datatype="http://www.w3.org/2001/XMLSchema#string">https://en.wikipedia.org/wiki/S%C3%A9millon</obo:IAO_0000119>
        <schema:image rdf:resource="https://upload.wikimedia.org/wikipedia/commons/thumb/2/27/Semillon_starting_to_get_noble_rot_at_Ch%C3%A2teau_Doisy-V%C3%A9drines%2C_Barsac%2C_Sauternes.jpg/160px-Semillon_starting_to_get_noble_rot_at_Ch%C3%A2teau_Doisy-V%C3%A9drines%2C_Barsac%2C_Sauternes.jpg"/>
        <oboInOwl:hasExactSynonym xml:lang="fr">Sémillon grape</oboInOwl:hasExactSynonym>
        <rdfs:label xml:lang="en">Semillon grape plant</rdfs:label>
    </owl:Class>
    


    <!-- http://purl.obolibrary.org/obo/FOODON_00002609 -->

    <owl:Class rdf:about="http://purl.obolibrary.org/obo/FOODON_00002609">
        <rdfs:subClassOf rdf:resource="http://purl.obolibrary.org/obo/FOODON_03310273"/>
        <rdfs:subClassOf>
            <owl:Class>
                <owl:intersectionOf rdf:parseType="Collection">
                    <owl:Restriction>
                        <owl:onProperty rdf:resource="http://purl.obolibrary.org/obo/RO_0001000"/>
                        <owl:someValuesFrom rdf:resource="http://purl.obolibrary.org/obo/FOODON_00002610"/>
                    </owl:Restriction>
                    <owl:Restriction>
                        <owl:onProperty rdf:resource="http://purl.obolibrary.org/obo/RO_0001000"/>
                        <owl:allValuesFrom rdf:resource="http://purl.obolibrary.org/obo/FOODON_00002610"/>
                    </owl:Restriction>
                </owl:intersectionOf>
            </owl:Class>
        </rdfs:subClassOf>
        <obo:IAO_0000114 rdf:resource="http://purl.obolibrary.org/obo/IAO_0000122"/>
        <obo:IAO_0000115 xml:lang="en">Glera wine is a white wine varietal produced only from Glera grapes. </obo:IAO_0000115>
        <obo:IAO_0000117 rdf:datatype="http://www.w3.org/2001/XMLSchema#string">Ginny Pichler</obo:IAO_0000117>
        <oboInOwl:hasExactSynonym xml:lang="en">Prosecco wine</oboInOwl:hasExactSynonym>
        <rdfs:label xml:lang="en">Glera wine</rdfs:label>
    </owl:Class>
    


    <!-- http://purl.obolibrary.org/obo/FOODON_00002610 -->

    <owl:Class rdf:about="http://purl.obolibrary.org/obo/FOODON_00002610">
        <rdfs:subClassOf rdf:resource="http://purl.obolibrary.org/obo/FOODON_03412121"/>
        <obo:IAO_0000114 rdf:resource="http://purl.obolibrary.org/obo/IAO_0000122"/>
        <obo:IAO_0000115 xml:lang="en">Glera is a white variety of grape of Slovenian origin, which was brought to the village of Prosecco from Slovenia&apos;s Karst region. Glera was, until 2009, mostly referred to as Prosecco. It is mainly cultivated for use in sparkling Italian wine styles.</obo:IAO_0000115>
        <obo:IAO_0000117 rdf:datatype="http://www.w3.org/2001/XMLSchema#string">Ginny Pichler</obo:IAO_0000117>
        <obo:IAO_0000119 rdf:datatype="http://www.w3.org/2001/XMLSchema#string">https://en.wikipedia.org/wiki/Glera_(grape)</obo:IAO_0000119>
        <schema:image rdf:resource="https://cdn1.wine-searcher.net/images/grape/glera-(prosecco)-392-1-1.jpg"/>
        <oboInOwl:hasExactSynonym xml:lang="en">Prosecco grape</oboInOwl:hasExactSynonym>
        <rdfs:label xml:lang="en">Glera grape plant</rdfs:label>
    </owl:Class>
    


    <!-- http://purl.obolibrary.org/obo/FOODON_00002611 -->

    <owl:Class rdf:about="http://purl.obolibrary.org/obo/FOODON_00002611">
        <rdfs:subClassOf rdf:resource="http://purl.obolibrary.org/obo/FOODON_03310273"/>
        <rdfs:subClassOf>
            <owl:Class>
                <owl:intersectionOf rdf:parseType="Collection">
                    <owl:Restriction>
                        <owl:onProperty rdf:resource="http://purl.obolibrary.org/obo/RO_0001000"/>
                        <owl:someValuesFrom rdf:resource="http://purl.obolibrary.org/obo/FOODON_00002610"/>
                    </owl:Restriction>
                    <owl:Restriction>
                        <owl:onProperty rdf:resource="http://purl.obolibrary.org/obo/RO_0001000"/>
                        <owl:allValuesFrom rdf:resource="http://purl.obolibrary.org/obo/FOODON_00002610"/>
                    </owl:Restriction>
                </owl:intersectionOf>
            </owl:Class>
        </rdfs:subClassOf>
        <obo:IAO_0000114 rdf:resource="http://purl.obolibrary.org/obo/IAO_0000122"/>
        <obo:IAO_0000115 xml:lang="en">Prosecco is an Italian white wine varietal produced primarily from Glera grapes, but other grape varieties may be included. Prosecco controlled designation of origin can be spumante (&quot;sparkling wine&quot;), frizzante (&quot;semi-sparkling wine&quot;), or tranquillo (&quot;still wine&quot;).</obo:IAO_0000115>
        <obo:IAO_0000117 rdf:datatype="http://www.w3.org/2001/XMLSchema#string">Ginny Pichler</obo:IAO_0000117>
        <obo:IAO_0000119 rdf:datatype="http://www.w3.org/2001/XMLSchema#string">https://en.wikipedia.org/wiki/Prosecco</obo:IAO_0000119>
        <schema:image rdf:resource="https://upload.wikimedia.org/wikipedia/commons/thumb/c/ce/Prosecco_di_Conegliano_bottle_and_glass.jpg/151px-Prosecco_di_Conegliano_bottle_and_glass.jpg"/>
        <oboInOwl:hasExactSynonym xml:lang="it"> frizzante </oboInOwl:hasExactSynonym>
        <oboInOwl:hasExactSynonym xml:lang="it"> tranquillo</oboInOwl:hasExactSynonym>
        <oboInOwl:hasExactSynonym xml:lang="it">spumante </oboInOwl:hasExactSynonym>
        <rdfs:label xml:lang="en">Prosecco wine</rdfs:label>
    </owl:Class>
    


    <!-- http://purl.obolibrary.org/obo/FOODON_00002612 -->

    <owl:Class rdf:about="http://purl.obolibrary.org/obo/FOODON_00002612">
        <rdfs:subClassOf rdf:resource="http://purl.obolibrary.org/obo/FOODON_03310272"/>
        <rdfs:subClassOf>
            <owl:Class>
                <owl:intersectionOf rdf:parseType="Collection">
                    <owl:Restriction>
                        <owl:onProperty rdf:resource="http://purl.obolibrary.org/obo/RO_0001000"/>
                        <owl:someValuesFrom rdf:resource="http://purl.obolibrary.org/obo/FOODON_00002613"/>
                    </owl:Restriction>
                    <owl:Restriction>
                        <owl:onProperty rdf:resource="http://purl.obolibrary.org/obo/RO_0001000"/>
                        <owl:allValuesFrom rdf:resource="http://purl.obolibrary.org/obo/FOODON_00002613"/>
                    </owl:Restriction>
                </owl:intersectionOf>
            </owl:Class>
        </rdfs:subClassOf>
        <obo:IAO_0000114 rdf:resource="http://purl.obolibrary.org/obo/IAO_0000122"/>
        <obo:IAO_0000115 xml:lang="en">Syrah wine is a white wine produced entirely from Syrah grapes.  The wines are often powerfully flavoured and full-bodied.</obo:IAO_0000115>
        <obo:IAO_0000117 rdf:datatype="http://www.w3.org/2001/XMLSchema#string">Ginny Pichler</obo:IAO_0000117>
        <obo:IAO_0000119 rdf:datatype="http://www.w3.org/2001/XMLSchema#string">https://en.wikipedia.org/wiki/Syrah#Shiraz_wines</obo:IAO_0000119>
        <schema:image rdf:resource="https://upload.wikimedia.org/wikipedia/commons/thumb/8/8e/Walla_walla_Syrah.jpg/179px-Walla_walla_Syrah.jpg"/>
        <rdfs:label xml:lang="en">Syrah wine</rdfs:label>
    </owl:Class>
    


    <!-- http://purl.obolibrary.org/obo/FOODON_00002613 -->

    <owl:Class rdf:about="http://purl.obolibrary.org/obo/FOODON_00002613">
        <rdfs:subClassOf rdf:resource="http://purl.obolibrary.org/obo/FOODON_03412121"/>
        <obo:IAO_0000114 rdf:resource="http://purl.obolibrary.org/obo/IAO_0000122"/>
        <obo:IAO_0000115 xml:lang="en">Syrah is a dark-skinned grape variety grown throughout the world and used primarily to produce red wine. In 1999, Syrah was found to be the offspring of two obscure grapes from southeastern France, Dureza and Mondeuse Blanche.</obo:IAO_0000115>
        <obo:IAO_0000117 rdf:datatype="http://www.w3.org/2001/XMLSchema#string">Ginny Pichler</obo:IAO_0000117>
        <obo:IAO_0000119 rdf:datatype="http://www.w3.org/2001/XMLSchema#string">https://en.wikipedia.org/wiki/Syrah</obo:IAO_0000119>
        <schema:image rdf:resource="https://upload.wikimedia.org/wikipedia/commons/thumb/e/eb/Shiraz_Grapes.jpg/320px-Shiraz_Grapes.jpg"/>
        <oboInOwl:hasExactSynonym xml:lang="en">Shiraz</oboInOwl:hasExactSynonym>
        <rdfs:label xml:lang="en">Syrah grape plant</rdfs:label>
    </owl:Class>
    


    <!-- http://purl.obolibrary.org/obo/FOODON_00002614 -->

    <owl:Class rdf:about="http://purl.obolibrary.org/obo/FOODON_00002614">
        <rdfs:subClassOf rdf:resource="http://purl.obolibrary.org/obo/FOODON_03310272"/>
        <rdfs:subClassOf>
            <owl:Class>
                <owl:intersectionOf rdf:parseType="Collection">
                    <owl:Restriction>
                        <owl:onProperty rdf:resource="http://purl.obolibrary.org/obo/RO_0001000"/>
                        <owl:someValuesFrom rdf:resource="http://purl.obolibrary.org/obo/FOODON_00002615"/>
                    </owl:Restriction>
                    <owl:Restriction>
                        <owl:onProperty rdf:resource="http://purl.obolibrary.org/obo/RO_0001000"/>
                        <owl:allValuesFrom rdf:resource="http://purl.obolibrary.org/obo/FOODON_00002615"/>
                    </owl:Restriction>
                </owl:intersectionOf>
            </owl:Class>
        </rdfs:subClassOf>
        <obo:IAO_0000114 rdf:resource="http://purl.obolibrary.org/obo/IAO_0000122"/>
        <obo:IAO_0000115 xml:lang="en">Tempranillo wine is a red wine varietal produced entirely from Tempranillo grapes.</obo:IAO_0000115>
        <obo:IAO_0000117 rdf:datatype="http://www.w3.org/2001/XMLSchema#string">Damion Dooley</obo:IAO_0000117>
        <obo:IAO_0000119 rdf:datatype="http://www.w3.org/2001/XMLSchema#string">https://en.wikipedia.org/wiki/Tempranillo</obo:IAO_0000119>
        <rdfs:label xml:lang="en">Tempranillo wine</rdfs:label>
    </owl:Class>
    


    <!-- http://purl.obolibrary.org/obo/FOODON_00002615 -->

    <owl:Class rdf:about="http://purl.obolibrary.org/obo/FOODON_00002615">
        <rdfs:subClassOf rdf:resource="http://purl.obolibrary.org/obo/FOODON_03412121"/>
        <obo:IAO_0000114 rdf:resource="http://purl.obolibrary.org/obo/IAO_0000122"/>
        <obo:IAO_0000115 xml:lang="en">Tempranillo is a black grape variety widely grown to make full-bodied red wines in its native Spain.</obo:IAO_0000115>
        <obo:IAO_0000117 rdf:datatype="http://www.w3.org/2001/XMLSchema#string">Damion Dooley</obo:IAO_0000117>
        <obo:IAO_0000119 rdf:datatype="http://www.w3.org/2001/XMLSchema#string">https://en.wikipedia.org/wiki/Tempranillo</obo:IAO_0000119>
        <oboInOwl:hasExactSynonym xml:lang="es"> Cencibel </oboInOwl:hasExactSynonym>
        <oboInOwl:hasExactSynonym xml:lang="pt"> Tinta Roriz</oboInOwl:hasExactSynonym>
        <oboInOwl:hasExactSynonym xml:lang="es"> Tinta del Pais</oboInOwl:hasExactSynonym>
        <oboInOwl:hasExactSynonym xml:lang="pt">Aragonez </oboInOwl:hasExactSynonym>
        <oboInOwl:hasExactSynonym xml:lang="es">Ull de Llebre </oboInOwl:hasExactSynonym>
        <rdfs:label xml:lang="en">Tempranillo grape plant</rdfs:label>
    </owl:Class>
    


    <!-- http://purl.obolibrary.org/obo/FOODON_00002617 -->

    <owl:Class rdf:about="http://purl.obolibrary.org/obo/FOODON_00002617">
        <rdfs:subClassOf rdf:resource="http://purl.obolibrary.org/obo/FOODON_03310272"/>
        <rdfs:subClassOf>
            <owl:Class>
                <owl:intersectionOf rdf:parseType="Collection">
                    <owl:Restriction>
                        <owl:onProperty rdf:resource="http://purl.obolibrary.org/obo/RO_0001000"/>
                        <owl:someValuesFrom rdf:resource="http://purl.obolibrary.org/obo/FOODON_00002618"/>
                    </owl:Restriction>
                    <owl:Restriction>
                        <owl:onProperty rdf:resource="http://purl.obolibrary.org/obo/RO_0001000"/>
                        <owl:allValuesFrom rdf:resource="http://purl.obolibrary.org/obo/FOODON_00002618"/>
                    </owl:Restriction>
                </owl:intersectionOf>
            </owl:Class>
        </rdfs:subClassOf>
        <obo:IAO_0000114 rdf:resource="http://purl.obolibrary.org/obo/IAO_0000122"/>
        <obo:IAO_0000115 xml:lang="en">Zinfandel wine is a red wine varietal produced entirely from Zinfandel grapes.  A classic wine is high in both alcohol and tannins, intensely flavored and deeply colored.</obo:IAO_0000115>
        <obo:IAO_0000117 rdf:datatype="http://www.w3.org/2001/XMLSchema#string">Ginny Pichler</obo:IAO_0000117>
        <obo:IAO_0000119 rdf:datatype="http://www.w3.org/2001/XMLSchema#string">https://www.wine-searcher.com/grape-391-primitivo</obo:IAO_0000119>
        <rdfs:label xml:lang="en">Zinfandel wine</rdfs:label>
    </owl:Class>
    


    <!-- http://purl.obolibrary.org/obo/FOODON_00002618 -->

    <owl:Class rdf:about="http://purl.obolibrary.org/obo/FOODON_00002618">
        <rdfs:subClassOf rdf:resource="http://purl.obolibrary.org/obo/FOODON_03412121"/>
        <obo:IAO_0000114 rdf:resource="http://purl.obolibrary.org/obo/IAO_0000122"/>
        <obo:IAO_0000115 xml:lang="en">Zinfandel is a variety of black-skinned wine grape.</obo:IAO_0000115>
        <obo:IAO_0000117 rdf:datatype="http://www.w3.org/2001/XMLSchema#string">Ginny Pichler</obo:IAO_0000117>
        <obo:IAO_0000119 rdf:datatype="http://www.w3.org/2001/XMLSchema#string">https://en.wikipedia.org/wiki/Zinfandel</obo:IAO_0000119>
        <schema:image rdf:resource="https://upload.wikimedia.org/wikipedia/commons/f/fc/Zinfandel_grapes.jpg"/>
        <oboInOwl:hasExactSynonym xml:lang="en">Primitivo</oboInOwl:hasExactSynonym>
        <rdfs:label xml:lang="en">Zinfandel grape plant</rdfs:label>
    </owl:Class>
    


    <!-- http://purl.obolibrary.org/obo/FOODON_00002619 -->

    <owl:Class rdf:about="http://purl.obolibrary.org/obo/FOODON_00002619">
        <rdfs:subClassOf rdf:resource="http://purl.obolibrary.org/obo/FOODON_03310272"/>
        <rdfs:subClassOf>
            <owl:Class>
                <owl:intersectionOf rdf:parseType="Collection">
                    <owl:Restriction>
                        <owl:onProperty rdf:resource="http://purl.obolibrary.org/obo/RO_0001000"/>
                        <owl:someValuesFrom rdf:resource="http://purl.obolibrary.org/obo/FOODON_00002620"/>
                    </owl:Restriction>
                    <owl:Restriction>
                        <owl:onProperty rdf:resource="http://purl.obolibrary.org/obo/RO_0001000"/>
                        <owl:allValuesFrom rdf:resource="http://purl.obolibrary.org/obo/FOODON_00002620"/>
                    </owl:Restriction>
                </owl:intersectionOf>
            </owl:Class>
        </rdfs:subClassOf>
        <obo:IAO_0000114 rdf:resource="http://purl.obolibrary.org/obo/IAO_0000122"/>
        <obo:IAO_0000115 xml:lang="en">Frappato wine is a red wine varietal produced entirely from Frappato grapes.  As a varietal, Frappato produces light bodied wines with a distinct grapey aroma.</obo:IAO_0000115>
        <obo:IAO_0000117 rdf:datatype="http://www.w3.org/2001/XMLSchema#string">Damion Dooley</obo:IAO_0000117>
        <obo:IAO_0000119 rdf:datatype="http://www.w3.org/2001/XMLSchema#string">https://en.wikipedia.org/wiki/Frappato</obo:IAO_0000119>
        <oboInOwl:hasExactSynonym xml:lang="it"> Frappato Nero di Vittoria </oboInOwl:hasExactSynonym>
        <oboInOwl:hasExactSynonym xml:lang="it"> Frappatu </oboInOwl:hasExactSynonym>
        <oboInOwl:hasExactSynonym xml:lang="it"> Frappatu di Vittoria </oboInOwl:hasExactSynonym>
        <oboInOwl:hasExactSynonym xml:lang="it"> Nerello</oboInOwl:hasExactSynonym>
        <oboInOwl:hasExactSynonym xml:lang="it"> Nerello di Catania </oboInOwl:hasExactSynonym>
        <oboInOwl:hasExactSynonym xml:lang="it"> Nero Capitano.</oboInOwl:hasExactSynonym>
        <oboInOwl:hasExactSynonym xml:lang="it">Frappato Nero </oboInOwl:hasExactSynonym>
        <rdfs:label xml:lang="en">Frappato wine</rdfs:label>
    </owl:Class>
    


    <!-- http://purl.obolibrary.org/obo/FOODON_00002620 -->

    <owl:Class rdf:about="http://purl.obolibrary.org/obo/FOODON_00002620">
        <rdfs:subClassOf rdf:resource="http://purl.obolibrary.org/obo/FOODON_03412121"/>
        <obo:IAO_0000114 rdf:resource="http://purl.obolibrary.org/obo/IAO_0000122"/>
        <obo:IAO_0000115 xml:lang="en">Frappato di Vittoria or Frappato is a red Italian wine grape variety planted primarily in Sicily.</obo:IAO_0000115>
        <obo:IAO_0000117 rdf:datatype="http://www.w3.org/2001/XMLSchema#string">Damion Dooley</obo:IAO_0000117>
        <obo:IAO_0000119 rdf:datatype="http://www.w3.org/2001/XMLSchema#string">https://en.wikipedia.org/wiki/Frappato</obo:IAO_0000119>
        <oboInOwl:hasExactSynonym xml:lang="it">Frappato di Vittoria</oboInOwl:hasExactSynonym>
        <rdfs:label xml:lang="en">Frappato grape plant</rdfs:label>
    </owl:Class>
    


    <!-- http://purl.obolibrary.org/obo/FOODON_00002621 -->

    <owl:Class rdf:about="http://purl.obolibrary.org/obo/FOODON_00002621">
        <rdfs:subClassOf rdf:resource="http://purl.obolibrary.org/obo/FOODON_03310272"/>
        <rdfs:subClassOf>
            <owl:Class>
                <owl:intersectionOf rdf:parseType="Collection">
                    <owl:Restriction>
                        <owl:onProperty rdf:resource="http://purl.obolibrary.org/obo/RO_0001000"/>
                        <owl:someValuesFrom rdf:resource="http://purl.obolibrary.org/obo/FOODON_00002622"/>
                    </owl:Restriction>
                    <owl:Restriction>
                        <owl:onProperty rdf:resource="http://purl.obolibrary.org/obo/RO_0001000"/>
                        <owl:allValuesFrom rdf:resource="http://purl.obolibrary.org/obo/FOODON_00002622"/>
                    </owl:Restriction>
                </owl:intersectionOf>
            </owl:Class>
        </rdfs:subClassOf>
        <obo:IAO_0000114 rdf:resource="http://purl.obolibrary.org/obo/IAO_0000122"/>
        <obo:IAO_0000115 xml:lang="en">Gamay noir wine is a red wine varietal produced entirely from Gamay grapes.</obo:IAO_0000115>
        <obo:IAO_0000117 rdf:datatype="http://www.w3.org/2001/XMLSchema#string">Damion Dooley</obo:IAO_0000117>
        <obo:IAO_0000119 rdf:datatype="http://www.w3.org/2001/XMLSchema#string">https://en.wikipedia.org/wiki/Gamay</obo:IAO_0000119>
        <rdfs:label xml:lang="en">Gamay noir wine</rdfs:label>
    </owl:Class>
    


    <!-- http://purl.obolibrary.org/obo/FOODON_00002622 -->

    <owl:Class rdf:about="http://purl.obolibrary.org/obo/FOODON_00002622">
        <rdfs:subClassOf rdf:resource="http://purl.obolibrary.org/obo/FOODON_03412121"/>
        <obo:IAO_0000114 rdf:resource="http://purl.obolibrary.org/obo/IAO_0000122"/>
        <obo:IAO_0000115 xml:lang="en">Gamay is a purple-colored grape variety used to make red wines, most notably grown in Beaujolais and in the Loire Valley around Tours.</obo:IAO_0000115>
        <obo:IAO_0000117 rdf:datatype="http://www.w3.org/2001/XMLSchema#string">Damion Dooley</obo:IAO_0000117>
        <obo:IAO_0000119 rdf:datatype="http://www.w3.org/2001/XMLSchema#string">https://en.wikipedia.org/wiki/Gamay</obo:IAO_0000119>
        <schema:image rdf:resource="https://upload.wikimedia.org/wikipedia/commons/3/38/Gamay.jpg"/>
        <oboInOwl:hasExactSynonym xml:lang="fr">Gamay Noir à Jus Blanc</oboInOwl:hasExactSynonym>
        <rdfs:label xml:lang="en">Gamay grape plant</rdfs:label>
    </owl:Class>
    


    <!-- http://purl.obolibrary.org/obo/FOODON_00002623 -->

    <owl:Class rdf:about="http://purl.obolibrary.org/obo/FOODON_00002623">
        <rdfs:subClassOf rdf:resource="http://purl.obolibrary.org/obo/FOODON_03310273"/>
        <rdfs:subClassOf>
            <owl:Class>
                <owl:intersectionOf rdf:parseType="Collection">
                    <owl:Restriction>
                        <owl:onProperty rdf:resource="http://purl.obolibrary.org/obo/RO_0001000"/>
                        <owl:someValuesFrom rdf:resource="http://purl.obolibrary.org/obo/FOODON_00002624"/>
                    </owl:Restriction>
                    <owl:Restriction>
                        <owl:onProperty rdf:resource="http://purl.obolibrary.org/obo/RO_0001000"/>
                        <owl:allValuesFrom rdf:resource="http://purl.obolibrary.org/obo/FOODON_00002624"/>
                    </owl:Restriction>
                </owl:intersectionOf>
            </owl:Class>
        </rdfs:subClassOf>
        <obo:IAO_0000114 rdf:resource="http://purl.obolibrary.org/obo/IAO_0000122"/>
        <obo:IAO_0000115 xml:lang="en">Gewürztraminerwine is a white wine varietal produced entirely from Gewürztraminer grapes.</obo:IAO_0000115>
        <obo:IAO_0000117 rdf:datatype="http://www.w3.org/2001/XMLSchema#string">Damion Dooley</obo:IAO_0000117>
        <obo:IAO_0000119 rdf:datatype="http://www.w3.org/2001/XMLSchema#string">https://en.wikipedia.org/wiki/Gew%C3%BCrztraminer</obo:IAO_0000119>
        <rdfs:label xml:lang="en">Gewürztraminer wine</rdfs:label>
    </owl:Class>
    


    <!-- http://purl.obolibrary.org/obo/FOODON_00002624 -->

    <owl:Class rdf:about="http://purl.obolibrary.org/obo/FOODON_00002624">
        <rdfs:subClassOf rdf:resource="http://purl.obolibrary.org/obo/FOODON_03412121"/>
        <obo:IAO_0000114 rdf:resource="http://purl.obolibrary.org/obo/IAO_0000122"/>
        <obo:IAO_0000115 xml:lang="en">Gewürztraminer is an aromatic wine grape variety, used in white wines, and performs best in cooler climates.</obo:IAO_0000115>
        <obo:IAO_0000117 rdf:datatype="http://www.w3.org/2001/XMLSchema#string">Damion Dooley</obo:IAO_0000117>
        <obo:IAO_0000119 rdf:datatype="http://www.w3.org/2001/XMLSchema#string">https://en.wikipedia.org/wiki/Gew%C3%BCrztraminer</obo:IAO_0000119>
        <schema:image rdf:resource="https://upload.wikimedia.org/wikipedia/en/thumb/1/11/Gewurztraminer_-_raisins_sur_pied_de_vigne.jpg/320px-Gewurztraminer_-_raisins_sur_pied_de_vigne.jpg"/>
        <oboInOwl:hasExactSynonym xml:lang="fr">Gewurztraminer</oboInOwl:hasExactSynonym>
        <oboInOwl:hasExactSynonym xml:lang="en">Gewürz</oboInOwl:hasExactSynonym>
        <rdfs:label xml:lang="en">Gewürztraminer grape plant</rdfs:label>
    </owl:Class>
    


    <!-- http://purl.obolibrary.org/obo/FOODON_00002625 -->

    <owl:Class rdf:about="http://purl.obolibrary.org/obo/FOODON_00002625">
        <rdfs:subClassOf rdf:resource="http://purl.obolibrary.org/obo/FOODON_03310272"/>
        <rdfs:subClassOf>
            <owl:Class>
                <owl:intersectionOf rdf:parseType="Collection">
                    <owl:Restriction>
                        <owl:onProperty rdf:resource="http://purl.obolibrary.org/obo/RO_0001000"/>
                        <owl:someValuesFrom rdf:resource="http://purl.obolibrary.org/obo/FOODON_00002626"/>
                    </owl:Restriction>
                    <owl:Restriction>
                        <owl:onProperty rdf:resource="http://purl.obolibrary.org/obo/RO_0001000"/>
                        <owl:allValuesFrom rdf:resource="http://purl.obolibrary.org/obo/FOODON_00002626"/>
                    </owl:Restriction>
                </owl:intersectionOf>
            </owl:Class>
        </rdfs:subClassOf>
        <obo:IAO_0000114 rdf:resource="http://purl.obolibrary.org/obo/IAO_0000122"/>
        <obo:IAO_0000115 xml:lang="en">Carignane wine is a red wine varietal produced entirely from Carignane grapes.</obo:IAO_0000115>
        <obo:IAO_0000117 rdf:datatype="http://www.w3.org/2001/XMLSchema#string">Damion Dooley</obo:IAO_0000117>
        <obo:IAO_0000119 rdf:datatype="http://www.w3.org/2001/XMLSchema#string">https://en.wikipedia.org/wiki/Carignan</obo:IAO_0000119>
        <rdfs:label xml:lang="en">Carignane wine</rdfs:label>
    </owl:Class>
    


    <!-- http://purl.obolibrary.org/obo/FOODON_00002626 -->

    <owl:Class rdf:about="http://purl.obolibrary.org/obo/FOODON_00002626">
        <rdfs:subClassOf rdf:resource="http://purl.obolibrary.org/obo/FOODON_03412121"/>
        <obo:IAO_0000114 rdf:resource="http://purl.obolibrary.org/obo/IAO_0000122"/>
        <obo:IAO_0000115 xml:lang="en">Carignan (also known as Carignane) is a red grape variety of Spanish origin that is more commonly found in French wine but is widely planted throughout the western Mediterranean and around the globe.</obo:IAO_0000115>
        <obo:IAO_0000117 rdf:datatype="http://www.w3.org/2001/XMLSchema#string">Damion Dooley</obo:IAO_0000117>
        <obo:IAO_0000119 rdf:datatype="http://www.w3.org/2001/XMLSchema#string">https://en.wikipedia.org/wiki/Carignan</obo:IAO_0000119>
        <schema:image rdf:resource="https://upload.wikimedia.org/wikipedia/commons/thumb/7/77/Carignan_Viala_et_Vermorel.jpg/415px-Carignan_Viala_et_Vermorel.jpg"/>
        <oboInOwl:hasExactSynonym xml:lang="it"> Bovale Grande</oboInOwl:hasExactSynonym>
        <oboInOwl:hasExactSynonym xml:lang="es"> Carinyena</oboInOwl:hasExactSynonym>
        <oboInOwl:hasExactSynonym xml:lang="es"> Mazuelo </oboInOwl:hasExactSynonym>
        <oboInOwl:hasExactSynonym xml:lang="es"> Samsó </oboInOwl:hasExactSynonym>
        <oboInOwl:hasExactSynonym xml:lang="it">Carignano </oboInOwl:hasExactSynonym>
        <oboInOwl:hasExactSynonym xml:lang="es">Cariñena </oboInOwl:hasExactSynonym>
        <rdfs:label xml:lang="en">Carignane grape plant</rdfs:label>
    </owl:Class>
    


    <!-- http://purl.obolibrary.org/obo/FOODON_00002627 -->

    <owl:Class rdf:about="http://purl.obolibrary.org/obo/FOODON_00002627">
        <rdfs:subClassOf rdf:resource="http://purl.obolibrary.org/obo/FOODON_03310272"/>
        <rdfs:subClassOf>
            <owl:Class>
                <owl:intersectionOf rdf:parseType="Collection">
                    <owl:Restriction>
                        <owl:onProperty rdf:resource="http://purl.obolibrary.org/obo/RO_0001000"/>
                        <owl:someValuesFrom rdf:resource="http://purl.obolibrary.org/obo/FOODON_00002628"/>
                    </owl:Restriction>
                    <owl:Restriction>
                        <owl:onProperty rdf:resource="http://purl.obolibrary.org/obo/RO_0001000"/>
                        <owl:allValuesFrom rdf:resource="http://purl.obolibrary.org/obo/FOODON_00002628"/>
                    </owl:Restriction>
                </owl:intersectionOf>
            </owl:Class>
        </rdfs:subClassOf>
        <obo:IAO_0000114 rdf:resource="http://purl.obolibrary.org/obo/IAO_0000122"/>
        <obo:IAO_0000115 xml:lang="en">Grenache wine is a red wine varietal produced entirely from Grenache grapes.</obo:IAO_0000115>
        <obo:IAO_0000117 rdf:datatype="http://www.w3.org/2001/XMLSchema#string">Damion Dooley</obo:IAO_0000117>
        <obo:IAO_0000119 rdf:datatype="http://www.w3.org/2001/XMLSchema#string">https://en.wikipedia.org/wiki/Grenache</obo:IAO_0000119>
        <rdfs:label xml:lang="en">Grenache wine</rdfs:label>
    </owl:Class>
    


    <!-- http://purl.obolibrary.org/obo/FOODON_00002628 -->

    <owl:Class rdf:about="http://purl.obolibrary.org/obo/FOODON_00002628">
        <rdfs:subClassOf rdf:resource="http://purl.obolibrary.org/obo/FOODON_03412121"/>
        <obo:IAO_0000114 rdf:resource="http://purl.obolibrary.org/obo/IAO_0000122"/>
        <obo:IAO_0000115 xml:lang="en">Grenache is one of the most widely planted red wine grape varieties in the world.</obo:IAO_0000115>
        <obo:IAO_0000117 rdf:datatype="http://www.w3.org/2001/XMLSchema#string">Damion Dooley</obo:IAO_0000117>
        <obo:IAO_0000119 rdf:datatype="http://www.w3.org/2001/XMLSchema#string">https://en.wikipedia.org/wiki/Grenache</obo:IAO_0000119>
        <schema:image rdf:resource="https://upload.wikimedia.org/wikipedia/commons/thumb/b/bd/Grenache_N.jpg/440px-Grenache_N.jpg"/>
        <oboInOwl:hasExactSynonym xml:lang="es">Garnacha</oboInOwl:hasExactSynonym>
        <rdfs:label xml:lang="en">Grenache grape plant</rdfs:label>
    </owl:Class>
    


    <!-- http://purl.obolibrary.org/obo/FOODON_00002629 -->

    <owl:Class rdf:about="http://purl.obolibrary.org/obo/FOODON_00002629">
        <rdfs:subClassOf rdf:resource="http://purl.obolibrary.org/obo/FOODON_03310272"/>
        <rdfs:subClassOf>
            <owl:Class>
                <owl:intersectionOf rdf:parseType="Collection">
                    <owl:Restriction>
                        <owl:onProperty rdf:resource="http://purl.obolibrary.org/obo/RO_0001000"/>
                        <owl:someValuesFrom rdf:resource="http://purl.obolibrary.org/obo/FOODON_00002630"/>
                    </owl:Restriction>
                    <owl:Restriction>
                        <owl:onProperty rdf:resource="http://purl.obolibrary.org/obo/RO_0001000"/>
                        <owl:allValuesFrom rdf:resource="http://purl.obolibrary.org/obo/FOODON_00002630"/>
                    </owl:Restriction>
                </owl:intersectionOf>
            </owl:Class>
        </rdfs:subClassOf>
        <obo:IAO_0000114 rdf:resource="http://purl.obolibrary.org/obo/IAO_0000122"/>
        <obo:IAO_0000115 xml:lang="en">Barbera wine is a red wine varietal produced entirely from Barbera grapes.</obo:IAO_0000115>
        <obo:IAO_0000117 rdf:datatype="http://www.w3.org/2001/XMLSchema#string">Damion Dooley</obo:IAO_0000117>
        <obo:IAO_0000119 rdf:datatype="http://www.w3.org/2001/XMLSchema#string">https://en.wikipedia.org/wiki/Barbera</obo:IAO_0000119>
        <rdfs:label xml:lang="en">Barbera wine</rdfs:label>
    </owl:Class>
    


    <!-- http://purl.obolibrary.org/obo/FOODON_00002630 -->

    <owl:Class rdf:about="http://purl.obolibrary.org/obo/FOODON_00002630">
        <rdfs:subClassOf rdf:resource="http://purl.obolibrary.org/obo/FOODON_03412121"/>
        <obo:IAO_0000114 rdf:resource="http://purl.obolibrary.org/obo/IAO_0000122"/>
        <obo:IAO_0000115 xml:lang="en">Barbera is a red Italian wine grape variety that, as of 2000, was the third most-planted red grape variety in Italy (after Sangiovese and Montepulciano). It produces good yields and is known for deep color, full body, low tannins and high levels of acid.</obo:IAO_0000115>
        <obo:IAO_0000117 rdf:datatype="http://www.w3.org/2001/XMLSchema#string">Damion Dooley</obo:IAO_0000117>
        <obo:IAO_0000119 rdf:datatype="http://www.w3.org/2001/XMLSchema#string">https://en.wikipedia.org/wiki/Barbera</obo:IAO_0000119>
        <rdfs:label xml:lang="en">Barbera grape plant</rdfs:label>
    </owl:Class>
    


    <!-- http://purl.obolibrary.org/obo/FOODON_00002631 -->

    <owl:Class rdf:about="http://purl.obolibrary.org/obo/FOODON_00002631">
        <rdfs:subClassOf rdf:resource="http://purl.obolibrary.org/obo/FOODON_00001211"/>
        <obo:IAO_0000114 rdf:resource="http://purl.obolibrary.org/obo/IAO_0000122"/>
        <obo:IAO_0000115 xml:lang="en">Tagliatelle is a traditional type of egg pasta from the Emilia-Romagna and Marche regions of Italy. Individual pieces of tagliatelle are long, flat ribbons that are similar in shape to fettuccine and are typically about 6.5 to 10 mm (0.26 to 0.39 in) wide.</obo:IAO_0000115>
        <obo:IAO_0000117 rdf:datatype="http://www.w3.org/2001/XMLSchema#string">Ginny Pichler</obo:IAO_0000117>
        <obo:IAO_0000119 rdf:datatype="http://www.w3.org/2001/XMLSchema#string">https://en.wikipedia.org/wiki/Tagliatelle</obo:IAO_0000119>
        <schema:image rdf:resource="https://upload.wikimedia.org/wikipedia/commons/thumb/0/02/Tagliatelles2.jpg/312px-Tagliatelles2.jpg"/>
        <rdfs:label xml:lang="en">tagliatelle</rdfs:label>
    </owl:Class>
    


    <!-- http://purl.obolibrary.org/obo/FOODON_00002632 -->

    <owl:Class rdf:about="http://purl.obolibrary.org/obo/FOODON_00002632">
        <rdfs:subClassOf rdf:resource="http://purl.obolibrary.org/obo/FOODON_00001211"/>
        <obo:IAO_0000114 rdf:resource="http://purl.obolibrary.org/obo/IAO_0000122"/>
        <obo:IAO_0000115 xml:lang="en">Tortellini are ring-shaped pasta, sometimes also described as &quot;navel shaped&quot;, hence their alternative name of &quot;belly button&quot; (ombelico). They are typically stuffed with a mix of meat (pork loin, raw prosciutto, Mortadella), and Parmigiano Reggiano cheese. </obo:IAO_0000115>
        <obo:IAO_0000117 rdf:datatype="http://www.w3.org/2001/XMLSchema#string">Ginny Pichler</obo:IAO_0000117>
        <obo:IAO_0000119 rdf:datatype="http://www.w3.org/2001/XMLSchema#string">https://en.wikipedia.org/wiki/Tortellini</obo:IAO_0000119>
        <schema:image rdf:resource="https://upload.wikimedia.org/wikipedia/commons/thumb/4/42/Tortellini_Bolognesi.jpg/320px-Tortellini_Bolognesi.jpg"/>
        <rdfs:label xml:lang="en">tortellini</rdfs:label>
    </owl:Class>
    


    <!-- http://purl.obolibrary.org/obo/FOODON_00002633 -->

    <owl:Class rdf:about="http://purl.obolibrary.org/obo/FOODON_00002633">
        <rdfs:subClassOf rdf:resource="http://purl.obolibrary.org/obo/FOODON_00001211"/>
        <obo:IAO_0000114 rdf:resource="http://purl.obolibrary.org/obo/IAO_0000122"/>
        <obo:IAO_0000115 xml:lang="en">Tortelloni are stuffed pasta, the same shape as tortellini, but larger. They are usually stuffed with ricotta cheese and leaf vegetables, such as spinach. </obo:IAO_0000115>
        <obo:IAO_0000117 rdf:datatype="http://www.w3.org/2001/XMLSchema#string">Shannon Russell</obo:IAO_0000117>
        <obo:IAO_0000119 rdf:datatype="http://www.w3.org/2001/XMLSchema#string">https://en.wikipedia.org/wiki/Tortelloni</obo:IAO_0000119>
        <schema:image rdf:resource="https://upload.wikimedia.org/wikipedia/commons/thumb/4/4c/Tortelloni_tomato_sauce1.JPG/275px-Tortelloni_tomato_sauce1.JPG"/>
        <rdfs:label xml:lang="en">tortelloni</rdfs:label>
    </owl:Class>
    


    <!-- http://purl.obolibrary.org/obo/FOODON_00002634 -->

    <owl:Class rdf:about="http://purl.obolibrary.org/obo/FOODON_00002634">
        <rdfs:subClassOf rdf:resource="http://purl.obolibrary.org/obo/FOODON_00001211"/>
        <obo:IAO_0000114 rdf:resource="http://purl.obolibrary.org/obo/IAO_0000122"/>
        <obo:IAO_0000115 xml:lang="en">Tortiglioni are a type of pasta, similar to rigatoni but larger and with deeper grooves which spiral around the pasta.</obo:IAO_0000115>
        <obo:IAO_0000117 rdf:datatype="http://www.w3.org/2001/XMLSchema#string">Lauren Tindale</obo:IAO_0000117>
        <obo:IAO_0000119 rdf:datatype="http://www.w3.org/2001/XMLSchema#string">https://en.wikipedia.org/wiki/Tortiglioni</obo:IAO_0000119>
        <schema:image rdf:resource="https://upload.wikimedia.org/wikipedia/commons/thumb/e/ef/Tortiglioni_closeup.png/320px-Tortiglioni_closeup.png"/>
        <rdfs:label xml:lang="en">tortiglioni</rdfs:label>
    </owl:Class>
    


    <!-- http://purl.obolibrary.org/obo/FOODON_00002635 -->

    <owl:Class rdf:about="http://purl.obolibrary.org/obo/FOODON_00002635">
        <rdfs:subClassOf rdf:resource="http://purl.obolibrary.org/obo/FOODON_00001211"/>
        <obo:IAO_0000114 rdf:resource="http://purl.obolibrary.org/obo/IAO_0000122"/>
        <obo:IAO_0000115 xml:lang="en">Fusilli are a variety of pasta that are formed into corkscrew or helical shapes. The word fusilli presumably comes from fuso (&quot;spindle&quot;), as traditionally it is &quot;spun&quot; by pressing and rolling a small rod over the thin strips of pasta to wind them around it in a corkscrew shape.</obo:IAO_0000115>
        <obo:IAO_0000117 rdf:datatype="http://www.w3.org/2001/XMLSchema#string">Shannon Russell</obo:IAO_0000117>
        <obo:IAO_0000119 rdf:datatype="http://www.w3.org/2001/XMLSchema#string">https://en.wikipedia.org/wiki/Fusilli</obo:IAO_0000119>
        <schema:image rdf:resource="https://en.wikipedia.org/wiki/Fusilli#/media/File:Fusilli.png"/>
        <oboInOwl:hasExactSynonym xml:lang="en">rotini</oboInOwl:hasExactSynonym>
        <rdfs:label xml:lang="en">fusilli</rdfs:label>
    </owl:Class>
    


    <!-- http://purl.obolibrary.org/obo/FOODON_00002636 -->

    <owl:Class rdf:about="http://purl.obolibrary.org/obo/FOODON_00002636">
        <rdfs:subClassOf rdf:resource="http://purl.obolibrary.org/obo/FOODON_00001211"/>
        <obo:IAO_0000114 rdf:resource="http://purl.obolibrary.org/obo/IAO_0000122"/>
        <obo:IAO_0000115 xml:lang="en">Conchiglie, commonly known as &quot;shells&quot; or &quot;seashells&quot; is a type of pasta. It is usually sold in the plain durum wheat variety. The shell shape of the pasta allows the sauce to adhere to it. </obo:IAO_0000115>
        <obo:IAO_0000117 rdf:datatype="http://www.w3.org/2001/XMLSchema#string">Emma Griffiths</obo:IAO_0000117>
        <obo:IAO_0000119 rdf:datatype="http://www.w3.org/2001/XMLSchema#string">https://en.wikipedia.org/wiki/Conchiglie</obo:IAO_0000119>
        <schema:image rdf:resource="https://upload.wikimedia.org/wikipedia/commons/thumb/2/20/Conchiglie_rigate.png/320px-Conchiglie_rigate.png"/>
        <rdfs:label xml:lang="en">conchiglie</rdfs:label>
    </owl:Class>
    


    <!-- http://purl.obolibrary.org/obo/FOODON_00002637 -->

    <owl:Class rdf:about="http://purl.obolibrary.org/obo/FOODON_00002637">
        <rdfs:subClassOf rdf:resource="http://purl.obolibrary.org/obo/FOODON_00001211"/>
        <obo:IAO_0000114 rdf:resource="http://purl.obolibrary.org/obo/IAO_0000122"/>
        <obo:IAO_0000115 xml:lang="en">Linguine is a type of pasta similar to fettuccine and trenette but elliptical in section rather than flat. It is about 4 millimetres in width, which is wider than spaghetti but not as wide as fettuccine. </obo:IAO_0000115>
        <obo:IAO_0000117 rdf:datatype="http://www.w3.org/2001/XMLSchema#string">Lauren Tindale</obo:IAO_0000117>
        <obo:IAO_0000119 rdf:datatype="http://www.w3.org/2001/XMLSchema#string">https://en.wikipedia.org/wiki/Linguine</obo:IAO_0000119>
        <schema:image rdf:resource="https://en.wikipedia.org/wiki/Linguine#/media/File:Linguine.jpg"/>
        <oboInOwl:hasExactSynonym xml:lang="en">trenette</oboInOwl:hasExactSynonym>
        <rdfs:label xml:lang="en">linguine</rdfs:label>
    </owl:Class>
    


    <!-- http://purl.obolibrary.org/obo/FOODON_00002638 -->

    <owl:Class rdf:about="http://purl.obolibrary.org/obo/FOODON_00002638">
        <rdfs:subClassOf rdf:resource="http://purl.obolibrary.org/obo/FOODON_00001211"/>
        <obo:IAO_0000114 rdf:resource="http://purl.obolibrary.org/obo/IAO_0000122"/>
        <obo:IAO_0000115 xml:lang="en">Penne is an extruded type of pasta with cylinder-shaped pieces, their ends cut at a bias. It is lexically related to Latin penna (meaning &quot;feather&quot; or &quot;quill&quot;), and was originally intended to imitate the then-ubiquitous fountain pen&apos;s steel nibs.</obo:IAO_0000115>
        <obo:IAO_0000117 rdf:datatype="http://www.w3.org/2001/XMLSchema#string">Emma Griffiths</obo:IAO_0000117>
        <obo:IAO_0000119 rdf:datatype="http://www.w3.org/2001/XMLSchema#string">https://en.wikipedia.org/wiki/Penne</obo:IAO_0000119>
        <schema:image rdf:resource="https://en.wikipedia.org/wiki/Penne#/media/File:Pennelisce_closeup.png"/>
        <rdfs:label xml:lang="en">penne</rdfs:label>
    </owl:Class>
    


    <!-- http://purl.obolibrary.org/obo/FOODON_00002639 -->

    <owl:Class rdf:about="http://purl.obolibrary.org/obo/FOODON_00002639">
        <rdfs:subClassOf rdf:resource="http://purl.obolibrary.org/obo/FOODON_00002577"/>
        <obo:IAO_0000114 rdf:resource="http://purl.obolibrary.org/obo/IAO_0000122"/>
        <obo:IAO_0000115 xml:lang="en">Zakynthos Wine is wine produced on the Greek island of Zakynthos (Zante) in the Ionian Sea. A wide array of native Ionian grape varieties have been planted on the island for centuries, and are most famously used to make the intensely flavored, highly acidic Verdea wine.</obo:IAO_0000115>
        <obo:IAO_0000117 rdf:datatype="http://www.w3.org/2001/XMLSchema#string">Damion Dooley</obo:IAO_0000117>
        <obo:IAO_0000119 rdf:datatype="http://www.w3.org/2001/XMLSchema#string">https://www.wine-searcher.com/regions-zakynthos</obo:IAO_0000119>
        <oboInOwl:hasExactSynonym xml:lang="en">zante wine</oboInOwl:hasExactSynonym>
        <rdfs:label xml:lang="en">Zakynthos Wine</rdfs:label>
    </owl:Class>
    


    <!-- http://purl.obolibrary.org/obo/FOODON_00002640 -->

    <owl:Class rdf:about="http://purl.obolibrary.org/obo/FOODON_00002640">
        <rdfs:subClassOf rdf:resource="http://purl.obolibrary.org/obo/FOODON_03412121"/>
        <obo:IAO_0000114 rdf:resource="http://purl.obolibrary.org/obo/IAO_0000122"/>
        <obo:IAO_0000115 xml:lang="en">The Cabernet Sauvignon grape plant originates from a cross between Cabernet Franc and Sauvignon blanc varieties. It produces Cabernet Sauvignon grapes, a red wine grape variety.</obo:IAO_0000115>
        <obo:IAO_0000117 rdf:datatype="http://www.w3.org/2001/XMLSchema#string">Emma Griffiths</obo:IAO_0000117>
        <obo:IAO_0000119 rdf:datatype="http://www.w3.org/2001/XMLSchema#string">https://en.wikipedia.org/wiki/Cabernet_Sauvignon</obo:IAO_0000119>
        <rdfs:label xml:lang="en">Cabernet Sauvignon grape plant</rdfs:label>
    </owl:Class>
    


    <!-- http://purl.obolibrary.org/obo/FOODON_00002641 -->

    <owl:Class rdf:about="http://purl.obolibrary.org/obo/FOODON_00002641">
        <rdfs:subClassOf rdf:resource="http://purl.obolibrary.org/obo/FOODON_00002577"/>
        <obo:IAO_0000114 rdf:resource="http://purl.obolibrary.org/obo/IAO_0000122"/>
        <obo:IAO_0000115 xml:lang="en">A Bordeaux wine is any wine produced in the Bordeaux region of southwest France.</obo:IAO_0000115>
        <obo:IAO_0000117 rdf:datatype="http://www.w3.org/2001/XMLSchema#string">Damion Dooley</obo:IAO_0000117>
        <obo:IAO_0000119 rdf:datatype="http://www.w3.org/2001/XMLSchema#string">https://en.wikipedia.org/wiki/Bordeaux_wine</obo:IAO_0000119>
        <oboInOwl:hasExactSynonym xml:lang="en-br">claret</oboInOwl:hasExactSynonym>
        <rdfs:label xml:lang="en">Bordeaux wine</rdfs:label>
    </owl:Class>
    


    <!-- http://purl.obolibrary.org/obo/FOODON_00002831 -->

    <owl:Class rdf:about="http://purl.obolibrary.org/obo/FOODON_00002831">
        <rdfs:subClassOf rdf:resource="http://purl.obolibrary.org/obo/FOODON_00001211"/>
        <obo:IAO_0000114 rdf:resource="http://purl.obolibrary.org/obo/IAO_0000122"/>
        <obo:IAO_0000115 xml:lang="en">Cannelloni are a cylindrical type of lasagna generally served baked with a filling and covered by a sauce in Italian cuisine.</obo:IAO_0000115>
        <obo:IAO_0000117 rdf:datatype="http://www.w3.org/2001/XMLSchema#string">Damion Dooley</obo:IAO_0000117>
        <obo:IAO_0000119 rdf:datatype="http://www.w3.org/2001/XMLSchema#string">https://en.wikipedia.org/wiki/Cannelloni</obo:IAO_0000119>
        <schema:image rdf:resource="https://upload.wikimedia.org/wikipedia/commons/thumb/6/6e/Cannelloni2.png/320px-Cannelloni2.png"/>
        <rdfs:label xml:lang="en">cannelloni</rdfs:label>
    </owl:Class>
    


    <!-- http://purl.obolibrary.org/obo/FOODON_00002863 -->

    <owl:Class rdf:about="http://purl.obolibrary.org/obo/FOODON_00002863">
        <rdfs:subClassOf rdf:resource="http://purl.obolibrary.org/obo/FOODON_03412121"/>
        <obo:IAO_0000114 rdf:resource="http://purl.obolibrary.org/obo/IAO_0000122"/>
        <obo:IAO_0000115 xml:lang="en">Blaufränkisch (German for blue Frankish) is a dark-skinned variety of grape used for red wine.</obo:IAO_0000115>
        <obo:IAO_0000117 rdf:datatype="http://www.w3.org/2001/XMLSchema#string">Damion Dooley</obo:IAO_0000117>
        <obo:IAO_0000119 rdf:datatype="http://www.w3.org/2001/XMLSchema#string">https://en.wikipedia.org/wiki/Blaufr%C3%A4nkisch</obo:IAO_0000119>
        <oboInOwl:hasExactSynonym xml:lang="ge"> Blauer Limberger </oboInOwl:hasExactSynonym>
        <oboInOwl:hasExactSynonym xml:lang="ge"> Blue Limberger</oboInOwl:hasExactSynonym>
        <oboInOwl:hasExactSynonym xml:lang="ge">Blaufränkisch grape</oboInOwl:hasExactSynonym>
        <oboInOwl:hasExactSynonym xml:lang="ge">lemberger </oboInOwl:hasExactSynonym>
        <rdfs:label xml:lang="en">Blaufränkisch grape plant</rdfs:label>
    </owl:Class>
    


    <!-- http://purl.obolibrary.org/obo/FOODON_00002864 -->

    <owl:Class rdf:about="http://purl.obolibrary.org/obo/FOODON_00002864">
        <rdfs:subClassOf rdf:resource="http://purl.obolibrary.org/obo/FOODON_03310272"/>
        <rdfs:subClassOf>
            <owl:Class>
                <owl:intersectionOf rdf:parseType="Collection">
                    <owl:Restriction>
                        <owl:onProperty rdf:resource="http://purl.obolibrary.org/obo/RO_0001000"/>
                        <owl:someValuesFrom rdf:resource="http://purl.obolibrary.org/obo/FOODON_00002863"/>
                    </owl:Restriction>
                    <owl:Restriction>
                        <owl:onProperty rdf:resource="http://purl.obolibrary.org/obo/RO_0001000"/>
                        <owl:allValuesFrom rdf:resource="http://purl.obolibrary.org/obo/FOODON_00002863"/>
                    </owl:Restriction>
                </owl:intersectionOf>
            </owl:Class>
        </rdfs:subClassOf>
        <obo:IAO_0000114 rdf:resource="http://purl.obolibrary.org/obo/IAO_0000122"/>
        <obo:IAO_0000115 xml:lang="en">Blaufränkisch wine is a red wine varietal produced entirely from Blaufränkisch grapes.</obo:IAO_0000115>
        <obo:IAO_0000117 rdf:datatype="http://www.w3.org/2001/XMLSchema#string">Damion Dooley</obo:IAO_0000117>
        <obo:IAO_0000119 rdf:datatype="http://www.w3.org/2001/XMLSchema#string">https://en.wikipedia.org/wiki/Blaufr%C3%A4nkisch</obo:IAO_0000119>
        <rdfs:label xml:lang="en">Blaufränkisch wine</rdfs:label>
    </owl:Class>
    


    <!-- http://purl.obolibrary.org/obo/FOODON_00002868 -->

    <owl:Class rdf:about="http://purl.obolibrary.org/obo/FOODON_00002868">
        <rdfs:subClassOf rdf:resource="http://purl.obolibrary.org/obo/FOODON_03412121"/>
        <obo:IAO_0000114 rdf:resource="http://purl.obolibrary.org/obo/IAO_0000122"/>
        <obo:IAO_0000115 xml:lang="en">Mourvèdre (also known as Mataró or Monastrell) is a red wine grape variety that is grown in many regions around the world including the Rhône and Provence regions of France, the Valencia and Jumilla denominaciones de origen of Spain, as well as the Balearic Islands, California and Washington and the Australian regions of South Australia and New South Wales, as well as South Africa.</obo:IAO_0000115>
        <obo:IAO_0000117 rdf:datatype="http://www.w3.org/2001/XMLSchema#string">Damion Dooley</obo:IAO_0000117>
        <schema:image rdf:resource="https://upload.wikimedia.org/wikipedia/commons/thumb/c/c6/Balzac_noir-mourvedre.jpg/451px-Balzac_noir-mourvedre.jpg"/>
        <oboInOwl:hasExactSynonym xml:lang="es">Monastrell</oboInOwl:hasExactSynonym>
        <oboInOwl:hasExactSynonym xml:lang="en">Mourvèdre grape | Mataró | Monastrell</oboInOwl:hasExactSynonym>
        <rdfs:label xml:lang="en">Mourvèdre grape plant</rdfs:label>
    </owl:Class>
    


    <!-- http://purl.obolibrary.org/obo/FOODON_00002869 -->

    <owl:Class rdf:about="http://purl.obolibrary.org/obo/FOODON_00002869">
        <rdfs:subClassOf rdf:resource="http://purl.obolibrary.org/obo/FOODON_03310272"/>
        <rdfs:subClassOf>
            <owl:Class>
                <owl:intersectionOf rdf:parseType="Collection">
                    <owl:Restriction>
                        <owl:onProperty rdf:resource="http://purl.obolibrary.org/obo/RO_0001000"/>
                        <owl:someValuesFrom rdf:resource="http://purl.obolibrary.org/obo/FOODON_00002868"/>
                    </owl:Restriction>
                    <owl:Restriction>
                        <owl:onProperty rdf:resource="http://purl.obolibrary.org/obo/RO_0001000"/>
                        <owl:allValuesFrom rdf:resource="http://purl.obolibrary.org/obo/FOODON_00002868"/>
                    </owl:Restriction>
                </owl:intersectionOf>
            </owl:Class>
        </rdfs:subClassOf>
        <obo:IAO_0000114 rdf:resource="http://purl.obolibrary.org/obo/IAO_0000122"/>
        <obo:IAO_0000117 rdf:datatype="http://www.w3.org/2001/XMLSchema#string">Damion Dooley</obo:IAO_0000117>
        <rdfs:label xml:lang="en">Mourvèdre wine</rdfs:label>
    </owl:Class>
    


    <!-- http://purl.obolibrary.org/obo/FOODON_03301014 -->

    <owl:Class rdf:about="http://purl.obolibrary.org/obo/FOODON_03301014"/>
    


    <!-- http://purl.obolibrary.org/obo/FOODON_03310272 -->

    <owl:Class rdf:about="http://purl.obolibrary.org/obo/FOODON_03310272"/>
    


    <!-- http://purl.obolibrary.org/obo/FOODON_03310273 -->

    <owl:Class rdf:about="http://purl.obolibrary.org/obo/FOODON_03310273"/>
    


    <!-- http://purl.obolibrary.org/obo/FOODON_03311123 -->

    <owl:Class rdf:about="http://purl.obolibrary.org/obo/FOODON_03311123">
        <rdfs:subClassOf rdf:resource="http://purl.obolibrary.org/obo/FOODON_00002577"/>
        <obo:IAO_0000114 rdf:resource="http://purl.obolibrary.org/obo/IAO_0000122"/>
        <obo:IAO_0000115 xml:lang="en">Chablis wine is a wine made in the Chablis region of France.</obo:IAO_0000115>
        <obo:IAO_0000117 rdf:datatype="http://www.w3.org/2001/XMLSchema#string">Emma Griffiths</obo:IAO_0000117>
        <obo:IAO_0000119 rdf:datatype="http://www.w3.org/2001/XMLSchema#string">https://en.wikipedia.org/wiki/Chablis_wine</obo:IAO_0000119>
        <rdfs:label xml:lang="en">Chablis wine</rdfs:label>
    </owl:Class>
    


    <!-- http://purl.obolibrary.org/obo/FOODON_03311270 -->

    <owl:Class rdf:about="http://purl.obolibrary.org/obo/FOODON_03311270">
        <rdfs:subClassOf rdf:resource="http://purl.obolibrary.org/obo/FOODON_00002577"/>
        <obo:IAO_0000114 rdf:resource="http://purl.obolibrary.org/obo/IAO_0000122"/>
        <obo:IAO_0000115 xml:lang="en">Beaujolais is a French Appellation d&apos;Origine Contrôlée (AOC) wine generally made of the Gamay grape which has a thin skin and is low in tannins.</obo:IAO_0000115>
        <obo:IAO_0000117 rdf:datatype="http://www.w3.org/2001/XMLSchema#string">Damion Dooley</obo:IAO_0000117>
        <obo:IAO_0000119 rdf:datatype="http://www.w3.org/2001/XMLSchema#string">https://en.wikipedia.org/wiki/Beaujolais</obo:IAO_0000119>
        <schema:image rdf:resource="https://upload.wikimedia.org/wikipedia/commons/thumb/d/d8/Carte_vignoble_beaujolais.png/356px-Carte_vignoble_beaujolais.png"/>
        <rdfs:label xml:lang="en">Beaujolais wine</rdfs:label>
    </owl:Class>
    


    <!-- http://purl.obolibrary.org/obo/FOODON_03412121 -->

    <owl:Class rdf:about="http://purl.obolibrary.org/obo/FOODON_03412121"/>
</rdf:RDF>



<!-- Generated by the OWL API (version 4.5.9.2019-02-01T07:24:44Z) https://github.com/owlcs/owlapi -->

